src/Lustre/Normalization/LNormalization.v
@@ -2,9 +2,9 @@ From Velus Require Import Common Ident.
 From Velus Require Import Operators Environment.
 From Velus Require Import CoindStreams.
 From Velus Require Import Lustre.LSyntax Lustre.LOrdered Lustre.LTyping Lustre.LClocking Lustre.LSemantics.
-From Velus Require Import Lustre.Normalization.Normalization Lustre.Normalization.Specification Lustre.Normalization.FullNorm.
-From Velus Require Import (* Lustre.Normalization.NTyping *) Lustre.Normalization.Correctness.
-From Velus Require Import Lustre.Normalization.Idempotence.
+From Velus Require Import Lustre.Normalization.Normalization.
+(* From Velus Require Import Lustre.Normalization.Correctness. *)
+(* From Velus Require Import Lustre.Normalization.Idempotence. *)
 
 Local Set Warnings "-masking-absolute-name".
 Module Type LNORMALIZATION
@@ -17,9 +17,9 @@ Module Type LNORMALIZATION
        (Import Clo : LCLOCKING Ids Op Syn)
        (Import Lord : LORDERED Ids Op Syn)
        (Import Sem : LSEMANTICS Ids Op OpAux Syn Lord Str).
-  Declare Module Norm : FULLNORM Ids Op OpAux Syn.
+  Declare Module Norm : NORMALIZATION Ids Op OpAux Syn.
   (* Declare Module Export Correct : CORRECTNESS Ids Op OpAux Str Syn Typ Clo Lord Sem Norm. *)
-  Declare Module Idempotence : IDEMPOTENCE Ids Op OpAux Syn Norm.
+  (* Declare Module Idempotence : IDEMPOTENCE Ids Op OpAux Syn Norm. *)
 End LNORMALIZATION.
 
 Module LNormalizationFun
@@ -33,7 +33,7 @@ Module LNormalizationFun
        (Lord : LORDERED Ids Op Syn)
        (Sem : LSEMANTICS Ids Op OpAux Syn Lord Str)
        <: LNORMALIZATION Ids Op OpAux Str Syn Typ Clo Lord Sem.
-  Module Norm := FullNormFun Ids Op OpAux Syn.
+  Module Norm := NormalizationFun Ids Op OpAux Syn.
   (* Module Export Correct := CorrectnessFun Ids Op OpAux Str Syn Typ Clo Lord Sem Norm. *)
-  Module Idempotence := IdempotenceFun Ids Op OpAux Syn Norm.
+  (* Module Idempotence := IdempotenceFun Ids Op OpAux Syn Norm. *)
 End LNormalizationFun.
