src/Lustre/Normalization/NormFby.v
@@ -1,0 +1,631 @@
+From Coq Require Import List Sorting.Permutation.
+Import List.ListNotations.
+Open Scope list_scope.
+Require Import Omega.
+
+From Velus Require Import Common Ident Environment.
+From Velus Require Import Operators.
+From Velus Require Import Lustre.LSyntax.
+From Velus Require Lustre.Normalization.Fresh.
+From Velus Require Import Lustre.Normalization.Untuple.
+
+(** * Putting FBYs into normalized form *)
+
+Local Set Warnings "-masking-absolute-name".
+Module Type NORMFBY
+       (Import Ids : IDS)
+       (Import Op : OPERATORS)
+       (OpAux : OPERATORS_AUX Op)
+       (Import Syn : LSYNTAX Ids Op)
+       (Import Unt : UNTUPLE Ids Op OpAux Syn).
+
+  Import Fresh Fresh.Fresh Fresh.Notations Facts Tactics.
+  Local Open Scope fresh_monad_scope.
+
+  (** Fresh ident generation keeping type annotations;
+      also retaining if the var is an init var or not *)
+  Definition FreshAnn A := Fresh A ((type * clock) * bool).
+
+  (** Add some whens on top of an expression *)
+  Fixpoint add_whens (e : exp) (ty : type) (cl : clock) :=
+    match cl with
+    | Cbase => e
+    | Con cl' clid b => Ewhen [(add_whens e ty cl')] clid b ([ty], (cl, None))
+    end.
+
+  (** Generate an init equation for a given clock `cl`; if the init equation for `cl` already exists,
+      just return the variable *)
+  Definition init_var_for_clock (cl : clock) : FreshAnn (ident * list equation) :=
+    fun st => match (find (fun '(_, ((ty, cl'), isinit)) => isinit && (cl' ==b cl) && (ty ==b Op.bool_type)) (st_anns st)) with
+           | Some (x, _) => ((x, []), st)
+           | None => let (x, st') := fresh_ident ((bool_type, cl), true) st in
+                    ((x, [([x], [Efby [add_whens (Econst true_const) bool_type cl]
+                                      [add_whens (Econst false_const) bool_type cl]
+                                      [(bool_type, (cl, None))]])]), st')
+           end.
+
+  Fixpoint is_constant (e : exp) : bool :=
+    match e with
+    | Econst _ => true
+    | Ewhen [e] _ _ ([ty], _) => is_constant e
+    | _ => false
+    end.
+
+  (** Generate a if-then-else equation for (0 fby e), and return an expression using it *)
+  Definition fby_iteexp (e0 : exp) (e : exp) (ann : ann) : FreshAnn (exp * list equation) :=
+    let '(ty, cl) := ann in
+    if (is_constant e0)
+    then ret (Efby [e0] [e] [ann], [])
+    else do (initid, eqs) <- init_var_for_clock (fst cl);
+         do px <- fresh_ident ((ty, fst cl), false);
+         ret (Eite (Evar initid (bool_type, (fst cl, Some initid))) [e0]
+                   [Evar px (ty, (fst cl, Some px))] ([ty], cl),
+              ([px], [Efby [add_whens (Econst (init_type ty)) ty (fst cl)] [e] [ann]])::eqs).
+
+  Definition fby_equation (to_cut : PS.t) (eq : equation) : FreshAnn (list equation) :=
+    match eq with
+    | ([x], [Efby [e0] [e] [ann]]) =>
+      let '(ty, (ck, _)) := ann in
+      do (fby, eqs) <- fby_iteexp e0 e ann;
+      if PS.mem x to_cut
+      then do x' <- fresh_ident ((ty, ck), false);
+           ret (([x], [Evar x' ann])::([x'], [fby])::eqs)
+      else ret (([x], [fby])::eqs)
+    | _ => ret [eq]
+    end.
+
+  Definition fby_equations (to_cut : PS.t) (eqs : list equation) : FreshAnn (list equation) :=
+    do eqs' <- map_bind (fby_equation to_cut) eqs;
+    ret (concat eqs').
+
+  (** Some initial properties *)
+
+  Local Ltac destruct_to_singl l :=
+    destruct l; [|destruct l]; auto.
+
+  Fact fby_equation_spec : forall to_cut xs es,
+      (exists x, exists e0, exists e, exists ann,
+                xs = [x] /\
+                es = [Efby [e0] [e] [ann]] /\
+                fby_equation to_cut (xs, es) =
+                (let '(ty, (ck, _)) := ann in
+                 do (fby, eqs) <- fby_iteexp e0 e ann;
+                 if PS.mem x to_cut
+                 then do x' <- fresh_ident ((ty, ck), false);
+                      ret (([x], [Evar x' ann])::([x'], [fby])::eqs)
+                 else ret (([x], [fby])::eqs)))
+      \/ fby_equation to_cut (xs, es) = (ret [(xs, es)]).
+  Proof.
+    intros *.
+    destruct_to_singl xs. destruct_to_singl es.
+    2: { right; simpl. destruct e; auto.
+         destruct_to_singl l. destruct_to_singl l0. destruct_to_singl l1. }
+    destruct e; auto.
+    destruct_to_singl l. destruct_to_singl l0. destruct_to_singl l1.
+    left. repeat eexists; eauto.
+  Qed.
+
+  (** *** Preservation of st_valid *)
+
+  Fact init_var_for_clock_st_valid : forall cl res st st' aft,
+      init_var_for_clock cl st = (res, st') ->
+      st_valid_after st aft ->
+      st_valid_after st' aft.
+  Proof.
+    intros * Hinit Hvalid.
+    unfold init_var_for_clock in Hinit.
+    repeat inv_bind.
+    destruct (find _ _).
+    - destruct p. inv Hinit. assumption.
+    - destruct (fresh_ident _ _) eqn:Hfresh. inv Hinit.
+      eapply fresh_ident_st_valid in Hfresh; eauto.
+  Qed.
+  Hint Resolve init_var_for_clock_st_valid.
+
+  Fact fby_iteexp_st_valid : forall e0 e a e' eqs' st st' aft,
+      fby_iteexp e0 e a st = (e', eqs', st') ->
+      st_valid_after st aft ->
+      st_valid_after st' aft.
+  Proof with eauto.
+    intros e0 e [ty cl] e' eqs' st st' aft Hfby Hvalid.
+    unfold fby_iteexp in Hfby.
+    destruct (is_constant e0); repeat inv_bind...
+  Qed.
+  Hint Resolve fby_iteexp_st_valid.
+
+  Fact fby_equation_st_valid : forall to_cut eq eqs' st st' aft,
+      fby_equation to_cut eq st = (eqs', st') ->
+      st_valid_after st aft ->
+      st_valid_after st' aft.
+  Proof.
+    intros to_cut [xs es] ? ? ? ? Hfby Hvalid.
+    specialize (fby_equation_spec to_cut xs es) as [[? [? [? [? [? [? Hspec]]]]]]|Hspec]; subst;
+      rewrite Hspec in Hfby; clear Hspec; [|repeat inv_bind; auto].
+    destruct x2 as [ty [ck name]]; repeat inv_bind.
+    destruct (PS.mem _ _); repeat inv_bind; auto.
+    - eapply fresh_ident_st_valid; eauto.
+      eapply fby_iteexp_st_valid with (a:=(ty, (ck, name))); unfold fby_iteexp; eauto.
+    - eapply fby_iteexp_st_valid with (a:=(ty, (ck, name))); unfold fby_iteexp; eauto.
+  Qed.
+
+  Fact fby_equations_st_valid : forall to_cut eqs eqs' st st' aft,
+      fby_equations to_cut eqs st = (eqs', st') ->
+      st_valid_after st aft ->
+      st_valid_after st' aft.
+  Proof.
+    intros * Hfby Hst.
+    unfold fby_equations in Hfby; repeat inv_bind.
+    eapply map_bind_st_valid in Hst; eauto.
+    solve_forall. eapply fby_equation_st_valid; eauto.
+  Qed.
+
+  (** *** Preservation of st_follows *)
+
+  Fact init_var_for_clock_st_follows : forall cl res st st',
+      init_var_for_clock cl st = (res, st') ->
+      st_follows st st'.
+  Proof.
+    intros cl res st st' Hinit.
+    unfold init_var_for_clock in Hinit.
+    repeat inv_bind.
+    destruct (find _ _).
+    - destruct p. inv Hinit. reflexivity.
+    - destruct (fresh_ident _ _) eqn:Hfresh. inv Hinit.
+      apply fresh_ident_st_follows in Hfresh. auto.
+  Qed.
+  Hint Resolve init_var_for_clock_st_follows.
+
+  Fact fby_iteexp_st_follows : forall e0 e ann res st st',
+      fby_iteexp e0 e ann st = (res, st') ->
+      st_follows st st'.
+  Proof.
+    intros e0 e [ty cl] res st st' Hfby.
+    unfold fby_iteexp in Hfby.
+    destruct (is_constant e0); repeat inv_bind.
+    - reflexivity.
+    - etransitivity; eauto.
+  Qed.
+  Hint Resolve fby_iteexp_st_follows.
+
+  (** *** The variables generated are a permutation of the ones contained in the state *)
+
+  Fact init_var_for_clock_vars_perm : forall cl id eqs st st',
+      init_var_for_clock cl st = ((id, eqs), st') ->
+      Permutation ((vars_defined eqs)++(st_ids st)) (st_ids st').
+  Proof.
+    intros cl id eqs st st' Hinit.
+    unfold init_var_for_clock in Hinit. repeat inv_bind.
+    destruct (find _ _).
+    - destruct p. inv Hinit. reflexivity.
+    - destruct (fresh_ident _ _) eqn:Hfresh. inv Hinit.
+      apply fresh_ident_vars_perm in Hfresh.
+      simpl. assumption.
+  Qed.
+
+  Fact fby_iteexp_vars_perm : forall e0 e ann e' eqs' st st',
+      fby_iteexp e0 e ann st = (e', eqs', st') ->
+      Permutation ((vars_defined eqs')++(st_ids st)) (st_ids st').
+  Proof.
+    intros ? ? [ty [ck name]] ? ? ? ? Hfby.
+    unfold fby_iteexp in Hfby. repeat inv_bind.
+    destruct (is_constant _); repeat inv_bind; simpl; eauto.
+    eapply init_var_for_clock_vars_perm in H; eauto.
+    eapply fresh_ident_vars_perm in H0.
+    rewrite <- H0, H; auto.
+  Qed.
+
+  Fact fby_equation_vars_perm : forall to_cut eq eqs' st st',
+      fby_equation to_cut eq st = (eqs', st') ->
+      Permutation ((vars_defined eqs')++(st_ids st)) ((vars_defined [eq])++(st_ids st')).
+  Proof.
+    intros to_cut [xs es] eqs' st st' Hfby.
+    specialize (fby_equation_spec to_cut xs es) as [[? [? [? [? [? [? Hspec]]]]]]|Hspec];
+      subst; rewrite Hspec in Hfby; clear Hspec.
+    - destruct x2 as [ty [ck name]]; repeat inv_bind.
+      eapply fby_iteexp_vars_perm with (ann:=(ty, (ck, name))) in H.
+      destruct (PS.mem _ _); repeat inv_bind; simpl.
+      + apply fresh_ident_vars_perm in H0.
+        rewrite H, <- H0; auto.
+      + rewrite H; auto.
+    - repeat inv_bind; simpl; auto.
+  Qed.
+
+  Fact fby_equations_vars_perm : forall to_cut eqs eqs' st st',
+      fby_equations to_cut eqs st = (eqs', st') ->
+      Permutation ((vars_defined eqs')++(st_ids st)) ((vars_defined eqs)++(st_ids st')).
+  Proof.
+    induction eqs; intros * Hnorm; unfold fby_equations in Hnorm; repeat inv_bind.
+    - reflexivity.
+    - assert (fby_equations to_cut eqs x1 = (concat x2, st')) as Hnorm'.
+      { unfold fby_equations. repeat inv_bind. repeat eexists; eauto.
+        inv_bind; eauto. } eapply IHeqs in Hnorm'; eauto.
+      eapply fby_equation_vars_perm in H; eauto; simpl in *.
+      repeat simpl_list.
+      rewrite Permutation_swap, H, Permutation_swap.
+      apply Permutation_app_head. assumption.
+  Qed.
+
+  (** *** Preservation of annotations *)
+
+  Fact fby_iteexp_annot : forall e0 e ann es' eqs' st st',
+      fby_iteexp e0 e ann st = (es', eqs', st') ->
+      annot es' = [ann].
+  Proof.
+    intros e0 e [ty [cl n]] es' eqs' st st' Hfby.
+    unfold fby_iteexp in Hfby.
+    destruct (is_constant e0); repeat inv_bind; reflexivity.
+  Qed.
+
+  (** *** Additional props *)
+
+  Fact init_var_for_clock_In : forall cl id eqs' st st',
+      init_var_for_clock cl st = (id, eqs', st') ->
+      In (id, (Op.bool_type, cl, true)) (st_anns st').
+  Proof.
+    intros cl id eqs' st st' Hinit.
+    unfold init_var_for_clock in Hinit.
+    destruct (find _ _) eqn:Hfind.
+    - destruct p; inv Hinit.
+      eapply find_some in Hfind. destruct Hfind as [Hin H].
+      destruct p as [[? ?] ?].
+      repeat rewrite Bool.andb_true_iff in H. destruct H as [[Hb Hcl] Hty].
+      rewrite OpAux.type_eqb_eq in Hty. rewrite Clocks.clock_eqb_eq in Hcl. subst. eauto.
+    - destruct (fresh_ident _ _) eqn:Hfresh. inv Hinit.
+      eapply fresh_ident_In in Hfresh; eauto.
+  Qed.
+
+  (** ** Specification of a normalized node *)
+
+  Inductive normalized_constant : exp -> Prop :=
+  | constant_Econst : forall c,
+      normalized_constant (Econst c)
+  | constant_Ewhen : forall e x b ty cl,
+      normalized_constant e ->
+      normalized_constant (Ewhen [e] x b ([ty], cl)).
+
+  Inductive normalized_equation : PS.t -> equation -> Prop :=
+  | normalized_eq_Eapp : forall out xs f es lann,
+      Forall normalized_lexp es ->
+      normalized_equation out (xs, [Eapp f es None lann])
+  | normalized_eq_Eapp_reset : forall out xs f es x ty cl lann,
+      Forall normalized_lexp es ->
+      normalized_equation out (xs, [Eapp f es (Some (Evar x (ty, cl))) lann])
+  | normalized_eq_Efby : forall out x e0 e ann,
+      ~PS.In x out ->
+      normalized_constant e0 ->
+      normalized_lexp e ->
+      normalized_equation out ([x], [Efby [e0] [e] [ann]])
+  | normalized_eq_cexp : forall out x e,
+      normalized_cexp e ->
+      normalized_equation out ([x], [e]).
+
+  Definition normalized_node (n : node) :=
+    Forall (normalized_equation (ps_from_list (List.map fst (n_out n)))) (n_eqs n).
+
+  Definition normalized_global (G : global) := Forall normalized_node G.
+
+  Hint Constructors normalized_constant normalized_equation.
+
+  (** *** Propagation of the weak_valid_after property *)
+
+  Fact init_var_for_clock_weak_valid : forall nck id st st' out,
+      init_var_for_clock nck st = (id, st') ->
+      weak_valid_after st out ->
+      weak_valid_after st' out.
+  Proof.
+    intros nck id st st' out Hinit Hval;
+      unfold init_var_for_clock in Hinit.
+    destruct find in Hinit.
+    - destruct p; inv Hinit; auto.
+    - destruct fresh_ident eqn:Hfresh.
+      inv Hinit; eauto.
+  Qed.
+  Local Hint Resolve init_var_for_clock_weak_valid.
+
+  Fact fby_iteexp_weak_valid : forall e0 e a e' eqs' st st' out,
+      fby_iteexp e0 e a st = (e', eqs', st') ->
+      weak_valid_after st out ->
+      weak_valid_after st' out.
+  Proof.
+    intros e0 e [ty cl] e' eqs' st st' out Hfby Hval;
+      unfold fby_iteexp in Hfby.
+    destruct (is_constant e0); repeat inv_bind; eauto.
+  Qed.
+  Local Hint Resolve fby_iteexp_weak_valid.
+
+  Fact fby_equation_weak_valid : forall eq eqs' st st' to_cut out,
+      fby_equation to_cut eq st = (eqs', st') ->
+      weak_valid_after st out ->
+      weak_valid_after st' out.
+  Proof.
+    intros * Hfby Hweak. destruct eq as [xs es].
+    specialize (fby_equation_spec to_cut xs es) as [[? [? [? [? [? [? Hspec]]]]]]|Hspec]; subst;
+      rewrite Hspec in Hfby; clear Hspec.
+    - destruct x2 as [ty [ck name]]; repeat inv_bind.
+      eapply fby_iteexp_weak_valid with (a:=(ty, (ck, name))) in H; eauto.
+      destruct (PS.mem _ _); repeat inv_bind; eauto.
+    - repeat inv_bind; auto.
+  Qed.
+
+  Fact fby_equations_weak_valid : forall eqs eqs' st st' to_cut out,
+      fby_equations to_cut eqs st = (eqs', st') ->
+      weak_valid_after st out ->
+      weak_valid_after st' out.
+  Proof.
+    intros * Hfby Hweak.
+    unfold fby_equations in Hfby; repeat inv_bind.
+    eapply map_bind_weak_valid in H; eauto.
+    solve_forall. eapply fby_equation_weak_valid; eauto.
+  Qed.
+
+  (** *** normalized_node implies untupled_node *)
+
+  Fact constant_normalized_lexp : forall e,
+      normalized_constant e ->
+      normalized_lexp e.
+  Proof.
+    intros e Hconst.
+    induction Hconst; auto.
+  Qed.
+
+  Fact normalized_eq_untupled_eq : forall to_cut eq,
+      normalized_equation to_cut eq ->
+      untupled_equation eq.
+  Proof.
+    intros * Hnormed. inv Hnormed; auto using constant_normalized_lexp.
+  Qed.
+
+  (** ** After normalization, equations and expressions are normalized *)
+
+  Fact add_whens_is_constant : forall ty cl e,
+      normalized_constant e ->
+      normalized_constant (add_whens e ty cl).
+  Proof.
+    induction cl; intros e Hcons; simpl.
+    - assumption.
+    - constructor. eauto.
+  Qed.
+
+  Fact add_whens_normalized_lexp : forall ty cl e,
+      normalized_lexp e ->
+      normalized_lexp (add_whens e ty cl).
+  Proof.
+    induction cl; intros e Hadd; simpl in Hadd.
+    - assumption.
+    - constructor. eauto.
+  Qed.
+
+  Fact is_constant_normalized_constant : forall e,
+      is_constant e = true <->
+      normalized_constant e.
+  Proof with eauto.
+    intros e. split; intros Hconst.
+    - induction e using exp_ind2; simpl in Hconst; try congruence.
+      + constructor.
+      + repeat (destruct es; try congruence).
+        inv H; inv H3.
+        destruct a.
+        repeat (destruct l; try congruence).
+        constructor...
+    - induction Hconst...
+  Qed.
+
+  Fact init_var_for_clock_normalized_eq : forall cl id eqs' out st st',
+      weak_valid_after st out ->
+      init_var_for_clock cl st = (id, eqs', st') ->
+      Forall (normalized_equation out) eqs'.
+  Proof.
+    intros cl id eqs' out st st' Hvalid Hinit.
+    unfold init_var_for_clock in Hinit.
+    destruct (find _ _).
+    - destruct p. inv Hinit. constructor.
+    - destruct (fresh_ident _ _) eqn:Hfresh. inv Hinit.
+      repeat constructor.
+      + eapply fresh_ident_weak_valid_nIn in Hfresh; eauto.
+      + apply add_whens_is_constant. auto.
+      + apply add_whens_normalized_lexp. auto.
+  Qed.
+
+  Fact fby_iteexp_normalized_eq : forall e0 e a e' eqs' out st st',
+      weak_valid_after st out ->
+      normalized_lexp e ->
+      fby_iteexp e0 e a st = (e', eqs', st') ->
+      Forall (normalized_equation out) eqs'.
+  Proof.
+    intros e0 e [ty cl] e' eqs' out st st' Hvalid He Hfby.
+    unfold fby_iteexp in Hfby.
+    destruct (is_constant e0); repeat inv_bind; constructor.
+    - assert (weak_valid_after x1 out) as Hvalid' by eauto.
+      constructor; auto.
+      + eapply fresh_ident_weak_valid_nIn in H0; eauto.
+      + eapply add_whens_is_constant; eauto.
+    - eapply init_var_for_clock_normalized_eq in H; eauto.
+  Qed.
+
+  Fact fby_equation_normalized_eq : forall out to_cut eq eqs' st st',
+      weak_valid_after st out ->
+      untupled_equation eq ->
+      PS.Subset out to_cut ->
+      fby_equation to_cut eq st = (eqs', st') ->
+      Forall (normalized_equation out) eqs'.
+  Proof.
+    intros out to_cut [xs es] eqs' st st' Hvalid Hunt Hsub Hfby.
+    inv Hunt; simpl in *.
+    - destruct_to_singl xs; repeat inv_bind; auto.
+    - destruct_to_singl xs; repeat inv_bind; auto.
+    - destruct ann0 as [ty [ck name]]; repeat inv_bind.
+      destruct (PS.mem _ _) eqn:Hmem; repeat inv_bind; constructor. 2:constructor.
+      3,5:eapply fby_iteexp_normalized_eq with (a:=(ty, (ck, name))); eauto.
+      2,3:destruct (is_constant e0) eqn:Hconst; repeat inv_bind.
+      1-5:repeat (constructor; eauto).
+      2,4:rewrite is_constant_normalized_constant in Hconst; eauto.
+      + eapply fresh_ident_weak_valid_nIn in H0; eauto.
+      + apply PSE.mem_4 in Hmem; auto.
+    - inv H0; repeat inv_bind; auto.
+      inv H; repeat inv_bind; auto.
+  Qed.
+
+  Fact fby_equations_normalized_eq : forall out to_cut eqs eqs' st st',
+      weak_valid_after st out ->
+      Forall untupled_equation eqs ->
+      PS.Subset out to_cut ->
+      fby_equations to_cut eqs st = (eqs', st') ->
+      Forall (normalized_equation out) eqs'.
+  Proof.
+    induction eqs; intros * Hvalid Hunt Hsub Hfby;
+      unfold fby_equations in Hfby; repeat inv_bind; simpl; auto.
+    inv Hunt.
+    eapply Forall_app; split.
+    - eapply fby_equation_normalized_eq in H; eauto.
+    - eapply IHeqs with (st:=x1) (st':=st'); eauto. 1:eapply fby_equation_weak_valid; eauto.
+      unfold fby_equations; repeat inv_bind.
+      repeat eexists; eauto. inv_bind; eauto.
+  Qed.
+
+  (** ** No anonymous names in a normalized node *)
+
+  Fact is_constant_no_fresh : forall e,
+      normalized_constant e ->
+      fresh_in e = [].
+  Proof with eauto.
+    intros e Hconst.
+    induction Hconst; simpl...
+    rewrite IHHconst...
+  Qed.
+
+  Lemma fby_equations_no_fresh : forall out to_cut eqs eqs' st st',
+      weak_valid_after st out ->
+      Forall untupled_equation eqs ->
+      PS.Subset out to_cut ->
+      fby_equations to_cut eqs st = (eqs', st') ->
+      anon_in_eqs eqs' = [].
+  Proof.
+    intros * Hweak Hunt Hsub Hfby.
+    eapply fby_equations_normalized_eq in Hfby; eauto.
+    eapply untupled_equations_no_anon.
+    solve_forall. eapply normalized_eq_untupled_eq; eauto.
+  Qed.
+
+  (** ** Normalization of a full node *)
+
+  Program Definition normfby_node (to_cut : PS.t) (n : node) (Hunt : untupled_node n) : node :=
+    let anon := anon_in_eqs (n_eqs n) in
+    let id0 := first_unused_ident (reserved++List.map fst (n_in n++n_vars n++n_out n++anon)) in
+    let eqs := fby_equations (PS.union to_cut (ps_from_list (map fst (n_out n)))) (n_eqs n) (init_st id0) in
+    let nvars := idty (st_anns (snd eqs)) in
+    {| n_name := n_name n;
+       n_hasstate := n_hasstate n;
+       n_in := n_in n;
+       n_out := n_out n;
+       n_vars := (n_vars n)++nvars;
+       n_eqs := fst eqs;
+       n_ingt0 := n_ingt0 n;
+       n_outgt0 := n_outgt0 n;
+    |}.
+  Next Obligation.
+    remember (first_unused_ident _) as id0.
+    remember (init_st _) as st.
+    remember (fby_equations _ _ _) as eqs. destruct eqs as [eqs st']. symmetry in Heqeqs.
+    specialize (n_defd n) as Hperm.
+    apply fby_equations_vars_perm in Heqeqs; simpl.
+    rewrite Permutation_app_comm, app_assoc, map_app, (Permutation_app_comm (n_out n)), <- Hperm, map_fst_idty.
+    rewrite <- Heqeqs, Heqst. unfold st_ids. rewrite init_st_anns, app_nil_r; auto.
+  Qed.
+  Next Obligation.
+    remember (first_unused_ident _) as id0.
+    remember (init_st _) as st.
+    remember (fby_equations _ _ _) as eqs. destruct eqs as [eqs st']. symmetry in Heqeqs.
+    assert (NoDup (map fst (n_in n ++ n_vars n ++ n_out n))) as Hndup.
+    { specialize (n_nodup n) as Hndup.
+      rewrite <- fst_NoDupMembers. repeat rewrite app_assoc in *. apply NoDupMembers_app_l in Hndup; auto. }
+    assert (st_valid_after st (PSP.of_list (map fst (n_in n ++ n_vars n ++ n_out n)))) as Hvalid.
+    { rewrite Heqst. eapply init_st_valid. symmetry in Heqid0. eapply first_unused_ident_gt in Heqid0.
+      rewrite PS_For_all_Forall.
+      eapply Forall_incl; eauto.
+      apply incl_tl, incl_tl.
+      rewrite ps_of_list_ps_to_list_Perm; eauto.
+      apply incl_map, incl_appr', incl_appr', incl_appl, incl_refl. }
+    assert (weak_valid_after st (PSP.of_list (map fst (n_out n)))) as Hweak.
+    { rewrite Heqst. eapply st_valid_weak_valid, init_st_valid. symmetry in Heqid0. eapply first_unused_ident_gt in Heqid0.
+      rewrite PS_For_all_Forall.
+      eapply Forall_incl; eauto.
+      apply incl_tl, incl_tl. intros ? Hin.
+      rewrite ps_of_list_ps_to_list in Hin. repeat simpl_In.
+      exists (i, (t, c)); split; auto. repeat rewrite in_app_iff in *; auto. }
+    simpl. erewrite fby_equations_no_fresh, app_nil_r. 2,3,5:eauto.
+    2:rewrite ps_from_list_ps_of_list; eapply PSP.union_subset_2.
+    eapply fby_equations_st_valid, st_valid_NoDup in Heqeqs; eauto.
+    rewrite ps_of_list_ps_to_list_Perm in Heqeqs; auto.
+    rewrite <- app_assoc, fst_NoDupMembers. repeat rewrite map_app in *.
+    unfold st_ids in Heqeqs. rewrite map_fst_idty, (app_assoc (map _ (n_vars _))), (Permutation_app_comm (map _ (n_vars _))),
+                             <- app_assoc, app_assoc, (Permutation_app_comm (map _ (n_in _))), <- app_assoc; auto.
+  Qed.
+  Admit Obligations.
+
+  Fixpoint normfby_global (G : global) (Hunt: Forall untupled_node G) : global.
+  Proof.
+    destruct G as [|hd tl].
+    - exact [].
+    - refine ((normfby_node PS.empty hd _)::(normfby_global tl _)).
+      + inv Hunt; eauto.
+      + inv Hunt; eauto.
+  Defined.
+
+  (** *** After normalization, a global is normalized *)
+
+  Fact normfby_node_normalized_node : forall n to_cut Hunt,
+      normalized_node (normfby_node to_cut n Hunt).
+  Proof.
+    intros *.
+    unfold normfby_node, normalized_node; simpl.
+    remember (first_unused_ident _) as id0.
+    remember (init_st _) as st.
+    remember (fby_equations _ _ _) as eqs. symmetry in Heqeqs. destruct eqs as [eqs st'].
+    eapply fby_equations_normalized_eq in Heqeqs; eauto.
+    2:rewrite ps_from_list_ps_of_list; eapply PSP.union_subset_2.
+    { rewrite Heqst. eapply st_valid_weak_valid, init_st_valid. symmetry in Heqid0. eapply first_unused_ident_gt in Heqid0.
+      rewrite PS_For_all_Forall.
+      eapply Forall_incl; eauto.
+      apply incl_tl, incl_tl. intros ? Hin.
+      rewrite ps_from_list_ps_of_list, ps_of_list_ps_to_list in Hin. repeat simpl_In.
+      exists (i, (t, c)); split; auto. repeat rewrite in_app_iff in *; auto. }
+  Qed.
+
+  Fact normfby_global_normalized_global : forall G Hunt,
+      normalized_global (normfby_global G Hunt).
+  Proof.
+    induction G; intros; simpl; constructor.
+    - eapply normfby_node_normalized_node.
+    - eapply IHG.
+  Qed.
+
+  (** *** normfby_global produces an equivalent global *)
+
+  Fact normfby_global_eq : forall G Hunt,
+      global_iface_eq G (normfby_global G Hunt).
+  Proof.
+    induction G; intros Hunt.
+    - reflexivity.
+    - simpl. apply global_iface_eq_cons; auto.
+  Qed.
+
+  Fact normfby_global_names : forall a G Hunt,
+      Forall (fun n => (n_name a <> n_name n)%type) G ->
+      Forall (fun n => (n_name a <> n_name n)%type) (normfby_global G Hunt).
+  Proof.
+    induction G; intros Hunt Hnames; simpl.
+    - constructor.
+    - inv Hnames.
+      constructor; eauto.
+  Qed.
+End NORMFBY.
+
+Module NormFbyFun
+       (Ids : IDS)
+       (Op : OPERATORS)
+       (OpAux : OPERATORS_AUX Op)
+       (Syn : LSYNTAX Ids Op)
+       (Unt : UNTUPLE Ids Op OpAux Syn)
+       <: NORMFBY Ids Op OpAux Syn Unt.
+  Include NORMFBY Ids Op OpAux Syn Unt.
+End NormFbyFun.
