src/Lustre/Normalization/Untuple.v
@@ -1,0 +1,2521 @@
+From Coq Require Import List Sorting.Permutation.
+Import List.ListNotations.
+Open Scope list_scope.
+Require Import Omega.
+
+From Velus Require Import Common Ident Environment.
+From Velus Require Import Operators.
+From Velus Require Import Lustre.LSyntax.
+From Velus Require Lustre.Normalization.Fresh.
+
+(** * Normalization procedure *)
+
+Local Set Warnings "-masking-absolute-name".
+Module Type UNTUPLE
+       (Import Ids : IDS)
+       (Import Op : OPERATORS)
+       (OpAux : OPERATORS_AUX Op)
+       (Import Syn : LSYNTAX Ids Op).
+
+  Import Fresh Fresh.Fresh Notations Facts Tactics.
+  Local Open Scope fresh_monad_scope.
+
+  (** Fresh ident generation keeping type annotations *)
+  Definition FreshAnn A := Fresh A (type * clock).
+
+  Definition hd_default (l : list exp) : exp :=
+    hd (Econst (init_type bool_type)) l.
+
+  Fixpoint idents_for_anns (anns : list ann) : FreshAnn (list (ident * ann)) :=
+    match anns with
+    | [] => ret []
+    | (ty, (cl, name))::tl => do x <- fresh_ident (ty, cl);
+                            do xs <- idents_for_anns tl;
+                            ret ((x, (ty, (cl, name)))::xs)
+    end.
+
+  Fact idents_for_anns_values: forall anns ids st st',
+      idents_for_anns anns st = (ids, st') ->
+      map snd ids = anns.
+  Proof.
+    induction anns; intros idents st st' Hanns; repeat inv_bind; auto.
+    destruct a as [ty [cl ?]]. repeat inv_bind.
+    specialize (IHanns _ _ _ H0); simpl.
+    f_equal; auto.
+  Qed.
+
+  Corollary idents_for_anns_length : forall anns idents st st',
+      idents_for_anns anns st = (idents, st') ->
+      length idents = length anns.
+  Proof.
+    intros.
+    apply idents_for_anns_values in H.
+    rewrite <- H. rewrite map_length; auto.
+  Qed.
+  Hint Resolve idents_for_anns_length.
+
+  (** Returns the identifiers for a list of annotations,
+      while applying clock substitutions *)
+  Fixpoint idents_for_anns' (anns : list ann) :=
+    match anns with
+    | [] => ret []
+    | (ty, (ck, None))::tl => do x <- fresh_ident (ty, ck);
+                            do xs <- idents_for_anns' tl;
+                            ret ((x, (ty, (ck, None)))::xs)
+    | (ty, (ck, Some x))::tl => do _ <- reuse_ident x (ty, ck);
+                              do xs <- idents_for_anns' tl;
+                              ret ((x, (ty, (ck, Some x)))::xs)
+    end.
+
+  Fact idents_for_anns'_values: forall anns idents st st',
+      idents_for_anns' anns st = (idents, st') ->
+      map snd idents = anns.
+  Proof.
+    induction anns; intros idents st st' Hanns; repeat inv_bind; simpl; auto.
+    destruct a as [ty [cl [name|]]]; repeat inv_bind; simpl;
+      specialize (IHanns _ _ _ H0);
+      f_equal; eauto.
+  Qed.
+
+  Corollary idents_for_anns'_length : forall anns ids st st',
+      idents_for_anns' anns st = (ids, st') ->
+      length ids = length anns.
+  Proof.
+    intros.
+    apply idents_for_anns'_values in H.
+    rewrite <- H. rewrite map_length; auto.
+  Qed.
+  Hint Resolve idents_for_anns'_length.
+
+  Definition normalize_fby (e0s : list exp) (es : list exp) (anns : list ann) :=
+    map (fun '((e0, e), a) => Efby [e0] [e] [a]) (combine (combine e0s es) anns).
+
+  Definition normalize_when ckid b es tys ck :=
+    map (fun '(e, ty) => Ewhen [e] ckid b ([ty], ck)) (combine es tys).
+
+  Definition normalize_merge ckid ets efs tys ck :=
+    map (fun '((e1, e2), ty) => Emerge ckid [e1] [e2] ([ty], ck)) (combine (combine ets efs) tys).
+
+  Definition normalize_ite e ets efs tys ck :=
+    map (fun '((et, ef), ty) => Eite e [et] [ef] ([ty], ck)) (combine (combine ets efs) tys).
+
+  Hint Unfold normalize_when normalize_merge normalize_ite.
+
+  Definition normalize_reset (e : exp) : FreshAnn (exp * list equation) :=
+    match e with
+    | Evar v ann => ret (Evar v ann, [])
+    | e => let '(ty, (cl, _)) := hd (bool_type, (Cbase, None)) (annot e) in
+          do x <- fresh_ident (ty, cl);
+          ret (Evar x (ty, (cl, Some x)), ([x], [e])::[])
+    end.
+
+  Lemma normalize_reset_spec : forall e,
+      (exists v, exists ann, e = Evar v ann /\ normalize_reset e = ret (Evar v ann, []))
+      \/ normalize_reset e = let '(ty, (cl, _)) := hd (bool_type, (Cbase, None)) (annot e) in
+                            do x <- fresh_ident (ty, cl);
+                            ret (Evar x (ty, (cl, Some x)), ([x], [e])::[]).
+  Proof. destruct e; eauto. Qed.
+
+  Fixpoint normalize_exp (is_control : bool) (e : exp) {struct e} : FreshAnn (list exp * list equation) :=
+    let normalize_exps := fun es => do (es, eqs) <- map_bind2 (normalize_exp false) es; ret (concat es, concat eqs) in
+    let normalize_controls := fun es => do (es, eqs) <- map_bind2 (normalize_exp true) es; ret (concat es, concat eqs) in
+    match e with
+    | Econst c => ret ([Econst c], [])
+    | Evar v ann => ret ([Evar v ann], [])
+    | Eunop op e1 ann =>
+      do (e1', eqs) <- normalize_exp false e1;
+      ret ([Eunop op (hd_default e1') ann], eqs)
+    | Ebinop op e1 e2 ann =>
+      do (e1', eqs1) <- normalize_exp false e1;
+      do (e2', eqs2) <- normalize_exp false e2;
+      ret ([Ebinop op (hd_default e1') (hd_default e2') ann], eqs1++eqs2)
+    | Ewhen es ckid b (tys, ck) =>
+      do (es', eqs) <- normalize_exps es;
+      ret (normalize_when ckid b es' tys ck, eqs)
+    | Emerge ckid es1 es2 (tys, cl) =>
+      do (es1', eqs1) <- normalize_controls es1;
+      do (es2', eqs2) <- normalize_controls es2;
+      let merges := normalize_merge ckid es1' es2' tys cl in
+      if is_control then
+        ret (merges, eqs1++eqs2)
+      else
+        do xs <- idents_for_anns (List.map (fun ty => (ty, cl)) tys);
+        ret (List.map (fun '(id, ann) => Evar id ann) xs,
+             (combine (List.map (fun '(id, _) => [id]) xs) (List.map (fun e => [e]) merges))++eqs1++eqs2)
+    | Eite e es1 es2 (tys, ck) =>
+      do (e', eqs0) <- normalize_exp false e;
+      do (es1', eqs1) <- normalize_controls es1;
+      do (es2', eqs2) <- normalize_controls es2;
+      let ites :=  normalize_ite (hd_default e') es1' es2' tys ck in
+      if is_control then
+        ret (ites, eqs0++eqs1++eqs2)
+      else
+        do xs <- idents_for_anns (List.map (fun ty => (ty, ck)) tys);
+        ret (List.map (fun '(id, ann) => Evar id ann) xs,
+             (combine (List.map (fun '(id, _) => [id]) xs) (List.map (fun e => [e]) ites))++eqs0++eqs1++eqs2)
+    | Efby e0s es anns =>
+      do (e0s', eqs1) <- normalize_exps e0s;
+      do (es', eqs2) <- normalize_exps es;
+      let fbys := normalize_fby e0s' es' anns in
+      do xs <- idents_for_anns anns;
+      ret (List.map (fun '(x, ann) => Evar x ann) xs,
+           (List.map (fun '((x, _), fby) => ([x], [fby])) (combine xs fbys))++eqs1++eqs2)
+    | Eapp f es r anns =>
+      do (es', eqs1) <- normalize_exps es;
+      do (r', eqs2) <- match r with
+                      | Some er => do (er, eqs1) <- normalize_exp false er;
+                                  do (er', eqs2) <- normalize_reset (hd_default er);
+                                  ret (Some er', eqs1++eqs2)
+                      | None => ret (None, [])
+                      end;
+      do xs <- idents_for_anns' anns;
+      ret (List.map (fun '(id, ann) => Evar id ann) xs,
+           (List.map fst xs, [Eapp f es' r' (List.map snd xs)])::eqs1++eqs2)
+    end.
+
+  Definition normalize_exps (es : list exp) :=
+    do (es, eqs) <- map_bind2 (normalize_exp false) es;
+    ret (concat es, concat eqs).
+
+  Definition normalize_rhs (e : exp) : FreshAnn (list exp * list equation) :=
+    match e with
+    | Eapp f es r anns =>
+      do (es', eqs1) <- normalize_exps es;
+      do (r', eqs2) <- match r with
+                      | Some er => do (er, eqs1) <- normalize_exp false er;
+                                  do (er', eqs2) <- normalize_reset (hd_default er);
+                                  ret (Some er', eqs1++eqs2)
+                      | None => ret (None, [])
+                      end;
+      ret ([Eapp f es' r' anns], eqs1++eqs2)
+    | Efby e0s es anns =>
+      do (e0s', eqs1) <- normalize_exps e0s;
+      do (es', eqs2) <- normalize_exps es;
+      let fbys := normalize_fby e0s' es' anns in
+      ret (fbys, eqs1++eqs2)
+    | _ => normalize_exp true e
+    end.
+
+  Definition normalize_rhss (es : list exp) :=
+    do (es, eqs) <- map_bind2 normalize_rhs es; ret (concat es, concat eqs).
+
+  Fixpoint combine_for_numstreams {B} (es : list exp) (vs : list B) :=
+    match es with
+    | [] => []
+    | hd::tl => let n := numstreams hd in
+                (hd, (firstn n vs))::(combine_for_numstreams tl (skipn n vs))
+    end.
+
+  Definition split_equation (eq : equation) : list equation :=
+    let (xs, es) := eq in
+    List.map (fun '(e, xs) => (xs, [e])) (combine_for_numstreams es xs).
+
+  Definition untuple_equation (e : equation) : FreshAnn (list equation) :=
+    let '(xs, es) := e in
+    do (es', eqs) <- normalize_rhss es;
+    ret ((split_equation (xs, es'))++eqs).
+
+  Definition untuple_equations (eqs : list equation) : FreshAnn (list equation) :=
+    do eqs <- map_bind untuple_equation eqs;
+    ret (concat eqs).
+
+  (** ** Some additional tactics *)
+
+  Definition default_ann : ann := (Op.bool_type, (Cbase, None)).
+
+  Ltac simpl_forall :=
+    repeat
+      match goal with
+      (* same *)
+      | |- Forall2 _ ?l1 ?l1 => apply Forall2_same
+      (* Get rid of maps *)
+      | H : Forall _ (map _ _) |- _ => rewrite Forall_map in H
+      | H : Forall2 _ (map _ _) _ |- _ => rewrite Forall2_map_1 in H
+      | H : Forall2 _ _ (map _ _) |- _ => rewrite Forall2_map_2 in H
+      | |- Forall _ (map _ _) => rewrite Forall_map
+      | |- Forall2 _ (map _ _) _ => rewrite Forall2_map_1
+      | |- Forall2 _ _ (map _ _) => rewrite Forall2_map_2
+      (* Get rid of combines *)
+      | |- Forall _ (combine _ _) => eapply Forall2_combine'
+      | |- Forall2 _ (combine _ _) _ => eapply Forall3_combine'1
+      (* Assemble Foralls *)
+      | H1 : Forall _ ?l, H2 : Forall _ ?l |- _ =>
+        eapply Forall_Forall in H1; [|eapply H2]; clear H2
+      | H1 : Forall2 _ ?l1 ?l2, H2 : Forall2 _ ?l1 ?l2 |- _ =>
+        eapply Forall2_Forall2 in H1; [|eapply H2]; clear H2
+      | H1 : Forall3 _ ?l1 ?l2 ?l3, H2 : Forall3 _ ?l1 ?l2 ?l3 |- _ =>
+        eapply Forall3_Forall3 in H1; [|eapply H2]; clear H2
+      (* Try to hyp Foralls in the same form as conclusion *)
+      | H : Forall _ ?l1 |- Forall2 _ ?l1 ?l2 =>
+        eapply Forall2_ignore2' with (ys:=l2) in H; try congruence
+      | H : Forall _ ?l2 |- Forall2 _ ?l1 ?l2 =>
+        eapply Forall2_ignore1' with (xs:=l1) in H; try congruence
+      | H : Forall2 _ ?l2 ?l3 |- Forall3 _ ?l1 ?l2 ?l3 =>
+        eapply Forall3_ignore1' with (xs:=l1) in H; try congruence
+      | H : Forall2 _ ?l1 ?l3 |- Forall3 _ ?l1 ?l2 ?l3 =>
+        eapply Forall3_ignore2' with (ys:=l2) in H; try congruence
+      | H : Forall2 _ ?l1 ?l2 |- Forall3 _ ?l1 ?l2 ?l3 =>
+        eapply Forall3_ignore3' with (zs:=l3) in H; try congruence
+      | H : Forall _ ?l1 |- Forall3 _ ?l1 ?l2 ?l3 =>
+        eapply Forall2_ignore2' with (ys:=l2) in H; try congruence
+      | H : Forall _ ?l2 |- Forall3 _ ?l1 ?l2 ?l3 =>
+        eapply Forall2_ignore1' with (xs:=l1) in H; try congruence
+      | H : Forall _ ?l3 |- Forall3 _ ?l1 ?l2 ?l3 =>
+        eapply Forall2_ignore1' with (xs:=l1) in H; try congruence
+      end; simpl in *; auto.
+
+  Ltac destruct_conjs :=
+    repeat
+      match goal with
+      | H: _ /\ _ |- _ => destruct H
+      | x: _ * _ |- _ => destruct x
+      end.
+
+  Ltac solve_forall :=
+    simpl_forall;
+    match goal with
+    | H: Forall _ ?l |- Forall _ ?l =>
+      eapply Forall_impl_In; [|eapply H]; clear H; intros; simpl in *
+    | H: Forall2 _ ?l1 ?l2 |- Forall2 _ ?l1 ?l2 =>
+      eapply Forall2_impl_In; [|eapply H]; clear H; intros; simpl in *
+    | H: Forall3 _ ?l1 ?l2 ?l3 |- Forall3 _ ?l1 ?l2 ?l3 =>
+      eapply Forall3_impl_In; [|eapply H]; clear H; intros; simpl in *
+    | |- Forall _ _ =>
+      eapply Forall_forall; intros
+    | _ => idtac
+    end; destruct_conjs; eauto.
+
+  Ltac simpl_In :=
+    match goal with
+    | x : ?t1 * ?t2 |- _ =>
+      destruct x
+    | H : In (?x1, ?x2) (combine ?l1 ?l2) |- _ =>
+      specialize (in_combine_l _ _ _ _ H) as ?; apply in_combine_r in H
+    | H : In ?x (map ?f ?l) |- _ =>
+      rewrite in_map_iff in H; destruct H as [? [? ?]]; subst
+    | |- In ?x (map ?f ?l) =>
+      rewrite in_map_iff
+    end.
+
+  (** ** Some additional facts *)
+
+  Fact combine_for_numstreams_In {B} : forall es (xs : list B) e x,
+      In (e, x) (combine_for_numstreams es xs) ->
+      In e es.
+  Proof.
+    induction es; intros xs e x Hin; simpl in Hin.
+    - inv Hin.
+    - destruct Hin.
+      + inv H. constructor; auto.
+      + right. eauto.
+  Qed.
+
+  (** ** Propagation of the st_valid_after property *)
+
+  Fact idents_for_anns_st_valid_after : forall anns res st st' aft,
+      idents_for_anns anns st = (res, st') ->
+      st_valid_after st aft ->
+      st_valid_after st' aft.
+  Proof.
+    induction anns; intros res st st' aft Hidforanns Hvalid;
+      repeat inv_bind.
+    - assumption.
+    - destruct a as [ty [cl name]]. repeat inv_bind.
+      eapply IHanns; eauto.
+  Qed.
+  Hint Resolve idents_for_anns_st_valid_after.
+
+  (** ** Propagation of the st_valid_reuse property *)
+
+  Fact idents_for_anns_st_valid_reuse : forall anns res st st' aft reusable,
+      idents_for_anns anns st = (res, st') ->
+      st_valid_reuse st aft reusable ->
+      st_valid_reuse st' aft reusable.
+  Proof.
+    induction anns; intros res st st' aft reuse Hidforanns Hvalid;
+      repeat inv_bind.
+    - assumption.
+    - destruct a as [ty [cl name]]. repeat inv_bind.
+      eapply IHanns; eauto.
+  Qed.
+  Hint Resolve idents_for_anns_st_valid_reuse.
+
+  Fact idents_for_anns'_st_valid : forall anns res st st' aft reusable,
+      NoDup (map fst (anon_streams anns)++PS.elements reusable) -> (* OK because of the n_dup property *)
+      idents_for_anns' anns st = (res, st') ->
+      st_valid_reuse st aft (ps_adds (map fst (anon_streams anns)) reusable) ->
+      st_valid_reuse st' aft reusable.
+  Proof with eauto.
+    induction anns; intros res st st' aft reusable HND Hidforanns Hvalid;
+      repeat inv_bind.
+    - assumption.
+    - destruct a as [ty [cl [name|]]]; repeat inv_bind; simpl in *;
+        eapply IHanns; eauto.
+      + inv HND; eauto.
+      + inv HND. destruct x.
+        eapply reuse_ident_st_valid_reuse in H; eauto.
+        * intro contra; apply H3.
+          rewrite <- In_PS_elements in contra.
+          rewrite Permutation_PS_elements_ps_adds' in contra...
+        * rewrite ps_add_adds_eq...
+  Qed.
+  Hint Resolve idents_for_anns'_st_valid.
+
+  Fact normalize_reset_st_valid : forall e res st st' aft reusable,
+      normalize_reset e st = (res, st') ->
+      st_valid_reuse st aft reusable ->
+      st_valid_reuse st' aft reusable.
+  Proof.
+    intros e res st st' aft reusable Hnorm Hvalid.
+    destruct (normalize_reset_spec e) as [[v [ann [He Hnorm']]]|Hnorm']; subst;
+      rewrite Hnorm' in Hnorm; clear Hnorm';
+        try (destruct (hd _ _) as [ty [cl _]]);
+        repeat inv_bind; eauto.
+  Qed.
+  Hint Resolve normalize_reset_st_valid.
+
+  Ltac ndup_simpl :=
+    repeat rewrite map_app, <- app_assoc in *.
+  Ltac ndup_l H :=
+    ndup_simpl;
+    rewrite Permutation_swap in H;
+    apply NoDup_app_r in H; auto.
+  Ltac ndup_r H :=
+    ndup_simpl;
+    apply NoDup_app_r in H; auto.
+
+  Fact map_bind2_st_valid_reuse' {B} :
+    forall (k : exp -> list (ident * B)) (f : exp -> FreshAnn (list exp * list equation)) es es' eqs' st st' aft reusable,
+      Forall (fun e =>
+                forall es' eqs' st st' aft reusable,
+                  NoDup (map fst (k e)++PS.elements reusable) ->
+                  f e st = (es', eqs', st') ->
+                  st_valid_reuse st aft (ps_adds (map fst (k e)) reusable) ->
+                  st_valid_reuse st' aft reusable) es ->
+      NoDup (map fst (concat (map k es))++PS.elements reusable) ->
+      map_bind2 f es st = (es', eqs', st') ->
+      st_valid_reuse st aft (ps_adds (map fst (concat (map k es))) reusable) ->
+      st_valid_reuse st' aft reusable.
+  Proof.
+    induction es; intros es' eqs' st st' aft reusable Hf Hnd Hmap Hvalid;
+      repeat inv_bind; auto.
+    inv Hf.
+    ndup_simpl.
+    assert (NoDup (map fst (k a)++PS.elements reusable)) by ndup_l Hnd.
+    assert (NoDup (map fst (concat (map k es))++PS.elements reusable)) by ndup_r Hnd.
+    rewrite ps_adds_app in Hvalid; eauto.
+    eapply IHes in H4; eauto. eapply H3; eauto.
+    rewrite Permutation_PS_elements_ps_adds'; eauto.
+  Qed.
+
+  Local Ltac solve_st_valid :=
+    match goal with
+    | H : map_bind2 _ _ _ = (_, _, ?st) |- st_valid_reuse ?st _ _ =>
+      eapply map_bind2_st_valid_reuse' in H; eauto; solve_forall
+    | H : normalize_reset _ _ = (_, _, ?st) |- st_valid_reuse ?st _ _ =>
+      eapply normalize_reset_st_valid; eauto
+    | H : idents_for_anns _ _ = (_, ?st) |- st_valid_reuse ?st _ _ =>
+      eapply idents_for_anns_st_valid_reuse; eauto
+    | H : idents_for_anns' _ _ = (_, ?st) |- st_valid_reuse ?st _ _ =>
+      eapply idents_for_anns'_st_valid; eauto
+    end.
+
+  Fact normalize_exp_st_valid : forall e is_control res st st' aft reusable,
+      NoDup (map fst (fresh_in e)++PS.elements reusable) ->
+      normalize_exp is_control e st = (res, st') ->
+      st_valid_reuse st aft (ps_adds (map fst (fresh_in e)) reusable) ->
+      st_valid_reuse st' aft reusable.
+  Proof with eauto.
+    induction e using exp_ind2; intros is_control res st st' aft reusable Hnd Hnorm Hvalid;
+      simpl in *.
+    - (* const *)
+      repeat inv_bind...
+    - (* var *)
+      repeat inv_bind...
+    - (* unop *)
+      repeat inv_bind...
+    - (* binop *)
+      repeat inv_bind. ndup_simpl.
+      assert (NoDup (map fst (fresh_in e1)++PS.elements reusable)) by ndup_l Hnd.
+      assert (NoDup (map fst (fresh_in e2)++PS.elements reusable)) by ndup_r Hnd.
+      rewrite ps_adds_app in *...
+      eapply IHe2... eapply IHe1...
+      rewrite Permutation_PS_elements_ps_adds'...
+    - (* fby *)
+      repeat inv_bind. ndup_simpl.
+      assert (NoDup (map fst (fresh_ins e0s)++PS.elements reusable)) by ndup_l Hnd.
+      assert (NoDup (map fst (fresh_ins es)++PS.elements reusable)) by ndup_r Hnd.
+      rewrite ps_adds_app in Hvalid... repeat solve_st_valid.
+      rewrite Permutation_PS_elements_ps_adds'; eauto.
+    - (* when *)
+      destruct a.
+      repeat inv_bind; repeat solve_st_valid.
+    - (* merge *)
+      destruct a. ndup_simpl.
+      assert (NoDup (map fst (fresh_ins ets)++PS.elements reusable)) by ndup_l Hnd.
+      assert (NoDup (map fst (fresh_ins efs)++PS.elements reusable)) by ndup_r Hnd.
+      destruct is_control; repeat inv_bind;
+        try rewrite ps_adds_app in *; repeat solve_st_valid;
+          rewrite Permutation_PS_elements_ps_adds'; eauto.
+    - (* ite *)
+      destruct a. ndup_simpl.
+      assert (NoDup (map fst (fresh_in e)++PS.elements reusable)) by (repeat ndup_l Hnd).
+      assert (NoDup (map fst (fresh_ins ets)++PS.elements reusable)) by (ndup_r Hnd; ndup_l Hnd).
+      assert (NoDup (map fst (fresh_ins efs)++PS.elements reusable)) by (repeat ndup_r Hnd).
+      assert (NoDup (map fst (fresh_ins ets)++map fst (fresh_ins efs)++PS.elements reusable)) by ndup_r Hnd.
+      destruct is_control; repeat inv_bind;
+        repeat rewrite ps_adds_app in Hvalid; repeat solve_st_valid.
+      2,4:eapply IHe; eauto.
+      1,2,3,4: repeat rewrite Permutation_PS_elements_ps_adds'; eauto.
+    - (* app *)
+      repeat inv_bind;
+        destruct ro; ndup_simpl;
+        repeat rewrite ps_adds_app in Hvalid; repeat inv_bind; repeat solve_st_valid...
+      2: (eapply H; eauto; repeat solve_st_valid).
+      2,3,5: repeat rewrite Permutation_PS_elements_ps_adds'; eauto.
+      1,2,3,4,5,6,7,8:repeat ndup_r Hnd.
+  Qed.
+  Hint Resolve normalize_exp_st_valid.
+
+  Fact normalize_rhs_st_valid : forall e res st st' aft reusable,
+      NoDup (map fst (anon_in e)++PS.elements reusable) ->
+      normalize_rhs e st = (res, st') ->
+      st_valid_reuse st aft (ps_adds (map fst (anon_in e)) reusable) ->
+      st_valid_reuse st' aft reusable.
+  Proof.
+    intros * Hnd Hnorm Hvalid.
+    destruct e; try (solve [eapply normalize_exp_st_valid in Hnorm; eauto]);
+      simpl in *; unfold normalize_exps in *.
+    - (* fby *)
+      ndup_simpl.
+      repeat inv_bind.
+      repeat rewrite ps_adds_app in Hvalid;
+        repeat solve_st_valid.
+      2: rewrite Permutation_PS_elements_ps_adds'; eauto.
+      1,2: ndup_r Hnd.
+    - (* app *)
+      repeat inv_bind.
+      destruct o; repeat inv_bind; ndup_simpl;
+        try rewrite ps_adds_app in Hvalid;
+        repeat solve_st_valid.
+      eapply normalize_exp_st_valid in H0; eauto. 2:solve_st_valid.
+      2:rewrite Permutation_PS_elements_ps_adds'; eauto.
+      1,2:ndup_r Hnd.
+  Qed.
+  Hint Resolve normalize_rhs_st_valid.
+
+  Fact untuple_equation_st_valid : forall e res st st' aft reusable,
+      NoDup (map fst (anon_in_eq e)++PS.elements reusable) ->
+      untuple_equation e st = (res, st') ->
+      st_valid_reuse st aft (ps_adds (map fst (anon_in_eq e)) reusable) ->
+      st_valid_reuse st' aft reusable.
+  Proof.
+    intros [xs es] * Hnd Hnorm Hvalid.
+    unfold anon_in_eq in Hnd.
+    simpl in *; unfold normalize_rhss in *; repeat inv_bind.
+    eapply map_bind2_st_valid_reuse' in H; eauto.
+    apply Forall_forall. intros; eauto.
+  Qed.
+  Hint Resolve untuple_equation_st_valid.
+
+  Fact untuple_equations_st_valid : forall eqs res st st' aft reusable,
+      NoDup (map fst (anon_in_eqs eqs)++PS.elements reusable) ->
+      untuple_equations eqs st = (res, st') ->
+      st_valid_reuse st aft (ps_adds (map fst (anon_in_eqs eqs)) reusable) ->
+      st_valid_reuse st' aft reusable.
+  Proof.
+    induction eqs; intros * Hndup Hnorm Hvalid;
+      unfold untuple_equations in Hnorm; repeat inv_bind; auto.
+    - unfold anon_in_eqs in *; simpl in *.
+      ndup_simpl.
+      rewrite ps_adds_app in Hvalid.
+      eapply IHeqs; eauto. 1:ndup_r Hndup.
+      unfold untuple_equations; repeat inv_bind; repeat eexists; eauto; inv_bind; eauto.
+      eapply untuple_equation_st_valid; eauto.
+      rewrite Permutation_PS_elements_ps_adds'; auto. ndup_r Hndup.
+  Qed.
+
+  (** ** Propagation of the st_follows property *)
+
+  Fact idents_for_anns_st_follows : forall anns res st st',
+      idents_for_anns anns st = (res, st') ->
+      st_follows st st'.
+  Proof.
+    induction anns; intros res st st' Hidforanns;
+      repeat inv_bind.
+    - reflexivity.
+    - destruct a as [ty [cl name]]. repeat inv_bind.
+      etransitivity; eauto.
+  Qed.
+  Hint Resolve idents_for_anns_st_follows.
+
+  Corollary idents_for_anns_incl : forall anns ids st st',
+      idents_for_anns anns st = (ids, st') ->
+      incl (List.map (fun '(id, (ty, (cl, _))) => (id, (ty, cl))) ids) (st_anns st').
+  Proof.
+    induction anns; intros ids st st' Hids; simpl in Hids; repeat inv_bind;
+      unfold incl; intros ? Hin; simpl in *; try destruct Hin.
+    destruct a as [ty [cl name]]. repeat inv_bind.
+    repeat simpl_In. inv H1. inv H2.
+    - inv H1.
+      apply fresh_ident_In in H.
+      apply idents_for_anns_st_follows in H0.
+      apply st_follows_incl in H0; auto.
+    - apply IHanns in H0.
+      apply H0. repeat simpl_In.
+      exists (i, (t, (c, o))); auto.
+  Qed.
+
+  Corollary idents_for_anns_incl_ids : forall anns ids st st',
+      idents_for_anns anns st = (ids, st') ->
+      incl (List.map fst ids) (st_ids st').
+  Proof.
+    intros.
+    eapply idents_for_anns_incl in H.
+    unfold st_ids, idty in *.
+    eapply incl_map with (f:=fst) in H.
+    repeat rewrite map_map in H; simpl in H.
+    replace (map (fun x => fst (let '(id, (ty, (cl, _))) := x in (id, (ty, cl)))) ids) with (map fst ids) in H.
+    2: { eapply map_ext. intros [? [? [? ?]]]; auto. }
+    assumption.
+  Qed.
+
+  Fact idents_for_anns'_st_follows : forall anns res st st',
+      idents_for_anns' anns st = (res, st') ->
+      st_follows st st'.
+  Proof.
+    induction anns; intros res st st' Hidforanns;
+      repeat inv_bind.
+    - reflexivity.
+    - destruct a as [ty [cl [name|]]]; repeat inv_bind;
+        [destruct x|]; etransitivity; eauto.
+  Qed.
+  Hint Resolve idents_for_anns'_st_follows.
+
+  Corollary idents_for_anns'_incl : forall anns ids st st',
+      idents_for_anns' anns st = (ids, st') ->
+      incl (List.map (fun '(id, (ty, (cl, _))) => (id, (ty, cl))) ids) (st_anns st').
+  Proof.
+    induction anns; intros ids st st' Hids; simpl in Hids; repeat inv_bind;
+      unfold incl; intros ? Hin; simpl in *; try destruct Hin.
+    destruct a as [ty [cl [name|]]]; repeat inv_bind; repeat simpl_In; inv H1; inv H2.
+    - inv H1. destruct x.
+      apply reuse_ident_In in H.
+      apply idents_for_anns'_st_follows in H0.
+      apply st_follows_incl in H0; auto.
+    - apply IHanns in H0.
+      apply H0. repeat simpl_In.
+      exists (i, (t, (c, o))); auto.
+    - inv H1.
+      apply fresh_ident_In in H.
+      apply idents_for_anns'_st_follows in H0.
+      apply st_follows_incl in H0; auto.
+    - apply IHanns in H0.
+      apply H0. repeat simpl_In.
+      exists (i, (t, (c, o))); auto.
+  Qed.
+
+  Corollary idents_for_anns'_incl_ids : forall anns ids st st',
+      idents_for_anns' anns st = (ids, st') ->
+      incl (List.map fst ids) (st_ids st').
+  Proof.
+    intros.
+    eapply idents_for_anns'_incl in H.
+    unfold st_ids, idty in *.
+    eapply incl_map with (f:=fst) in H.
+    repeat rewrite map_map in H; simpl in H.
+    replace (map (fun x => fst (let '(id, (ty, (cl, _))) := x in (id, (ty, cl)))) ids) with (map fst ids) in H.
+    2: { eapply map_ext. intros [? [? [? ?]]]; auto. }
+    assumption.
+  Qed.
+
+  Fact normalize_reset_st_follows : forall e res st st',
+      normalize_reset e st = (res, st') ->
+      st_follows st st'.
+  Proof.
+    intros e res st st' Hnorm.
+    destruct (normalize_reset_spec e) as [[v [ann [He Hnorm']]]|Hnorm']; subst;
+      repeat inv_bind.
+    - reflexivity.
+    - rewrite Hnorm' in Hnorm; clear Hnorm'.
+      destruct (hd _ _) as [ty [cl _]].
+      repeat inv_bind. eauto.
+  Qed.
+  Hint Resolve normalize_reset_st_follows.
+
+  Local Ltac solve_st_follows' :=
+    match goal with
+    | |- st_follows ?st ?st =>
+      reflexivity
+    | H : st_follows ?st1 ?st2 |- st_follows ?st1 _ =>
+      etransitivity; [eapply H |]
+    | H : fresh_ident _ ?st = _ |- st_follows ?st _ =>
+      etransitivity; [ eapply fresh_ident_st_follows in H; eauto | ]
+    | H : reuse_ident _ _ ?st = _ |- st_follows ?st _ =>
+      etransitivity; [ eapply reuse_ident_st_follows in H; eauto | ]
+    | H : idents_for_anns _ ?st = _ |- st_follows ?st _ =>
+      etransitivity; [ eapply idents_for_anns_st_follows in H; eauto | ]
+    | H : idents_for_anns' _ ?st = _ |- st_follows ?st _ =>
+      etransitivity; [ eapply idents_for_anns'_st_follows in H; eauto | ]
+    | H : normalize_reset _ ?st = _ |- st_follows ?st _ =>
+      etransitivity; [ eapply normalize_reset_st_follows in H; eauto | ]
+    | H : map_bind2 _ _ ?st = _ |- st_follows ?st _ =>
+      etransitivity; [ eapply map_bind2_st_follows in H; eauto; solve_forall | ]
+    end.
+
+  Fact normalize_exp_st_follows : forall e is_control res st st',
+      normalize_exp is_control e st = (res, st') ->
+      st_follows st st'.
+  Proof with eauto.
+    induction e using exp_ind2; intros is_control res st st' Hnorm;
+      simpl in Hnorm.
+    - (* const *)
+      repeat inv_bind; reflexivity.
+    - (* var *)
+      repeat inv_bind; reflexivity.
+    - (* unop *)
+      repeat inv_bind...
+    - (* binop *)
+      repeat inv_bind; etransitivity...
+    - (* fby *)
+      repeat inv_bind; repeat solve_st_follows'.
+    - (* when *)
+      destruct a.
+      repeat inv_bind; repeat solve_st_follows'.
+    - (* merge *)
+      destruct a.
+      destruct is_control; repeat inv_bind; repeat solve_st_follows'.
+    - (* ite *)
+      destruct a.
+      destruct is_control; repeat inv_bind;
+        (etransitivity; [ eapply IHe; eauto | repeat solve_st_follows' ]).
+    - (* app *)
+      destruct ro; repeat inv_bind; [eapply H in H2|]; repeat solve_st_follows'.
+  Qed.
+  Hint Resolve normalize_exp_st_follows.
+
+  Corollary normalize_exps_st_follows : forall es res st st',
+      normalize_exps es st = (res, st') ->
+      st_follows st st'.
+  Proof.
+    intros es res st st' Hnorm.
+    unfold normalize_exps in Hnorm. repeat inv_bind.
+    eapply map_bind2_st_follows; eauto.
+    rewrite Forall_forall; intros; eauto.
+  Qed.
+
+  Fact normalize_rhs_st_follows : forall e res st st',
+      normalize_rhs e st = (res, st') ->
+      st_follows st st'.
+  Proof.
+    intros * Hnorm.
+    destruct e; try (solve [eapply normalize_exp_st_follows; eauto]);
+      simpl in Hnorm; unfold normalize_exps in *.
+    - (* fby *)
+      repeat inv_bind;
+        repeat solve_st_follows';
+        eapply Forall_forall; intros; eauto.
+    - (* app *)
+      destruct o; repeat inv_bind; [eapply normalize_exp_st_follows in H0|]; repeat solve_st_follows'.
+  Qed.
+  Hint Resolve normalize_rhs_st_follows.
+
+  Corollary normalize_rhss_st_follows : forall es res st st',
+      normalize_rhss es st = (res, st') ->
+      st_follows st st'.
+  Proof.
+    intros * Hnorm.
+    unfold normalize_rhss in Hnorm; repeat inv_bind.
+    repeat solve_st_follows'.
+  Qed.
+  Hint Resolve normalize_rhss_st_follows.
+
+  Fact untuple_equation_st_follows : forall e res st st',
+      untuple_equation e st = (res, st') ->
+      st_follows st st'.
+  Proof.
+    intros [xs es] * Hnorm.
+    simpl in *; repeat inv_bind; eauto.
+  Qed.
+  Hint Resolve untuple_equation_st_follows.
+
+  Fact untuple_equations_st_follows : forall eqs res st st',
+      untuple_equations eqs st = (res, st') ->
+      st_follows st st'.
+  Proof.
+    intros * Hnorm.
+    unfold untuple_equations in Hnorm; repeat inv_bind.
+    eapply map_bind_st_follows; eauto.
+    solve_forall.
+  Qed.
+
+  Ltac solve_st_follows :=
+    match goal with
+    | |- st_follows ?st ?st => reflexivity
+    | H : normalize_exp _ _ ?st = _ |- st_follows ?st _ =>
+      etransitivity; [ eapply normalize_exp_st_follows in H; eauto |]
+    | H : normalize_exps _ ?st = _ |- st_follows ?st _ =>
+      etransitivity; [ eapply normalize_exps_st_follows in H; eauto |]
+    | H : normalize_rhs _ _ ?st = _ |- st_follows ?st _ =>
+      etransitivity; [ eapply normalize_rhs_st_follows in H; eauto |]
+    | H : normalize_rhss _ _ ?st = _ |- st_follows ?st _ =>
+      etransitivity; [ eapply normalize_rhss_st_follows in H; eauto |]
+    | H : untuple_equation _ _ ?st = _ |- st_follows ?st _ =>
+      etransitivity; [ eapply untuple_equation_st_follows in H; eauto |]
+    | H : untuple_equations _ _ ?st = _ |- st_follows ?st _ =>
+      etransitivity; [ eapply untuple_equations_st_follows in H; eauto |]
+    | _ => solve_st_follows'
+    end.
+
+  (** ** Some helpful tactics *)
+
+  (** Simplify an expression with maps and other stuff... *)
+  Ltac simpl_list :=
+    unfold normalize_when, normalize_merge, normalize_ite in *;
+    simpl in *;
+    match goal with
+    (* annots, clocksof and typesof are just plurals *)
+    | H : context c [annots ?es] |- _ => unfold annots in H
+    | |- context c [annots ?es] => unfold annots
+    | H : context c [typesof ?es] |- _ => unfold typesof in H
+    | |- context c [typesof ?es] => unfold typesof
+    | H : context c [clocksof ?es] |- _ => unfold clocksof in H
+    | |- context c [clocksof ?es] => unfold clocksof
+    | H : context c [vars_defined ?es] |- _ => unfold vars_defined in H
+    | |- context c [vars_defined ?es] => unfold vars_defined
+    (* flat_map, map_map, map_app, concat_app *)
+    | H: context c [flat_map ?f ?l] |- _ => rewrite flat_map_concat_map in H
+    | |- context c [flat_map ?f ?l] => rewrite flat_map_concat_map
+    | H: context c [map ?f (map ?g ?l)] |- _ => rewrite map_map in H
+    | |- context c [map ?f (map ?g ?l)] => rewrite map_map
+    | H: context c [map ?f (app ?l1 ?l2)] |- _ => rewrite map_app in H
+    | |- context c [map ?f (app ?l1 ?l2)] => rewrite map_app
+    | H: context c [concat (app ?l1 ?l2)] |- _ => rewrite concat_app in H
+    | |- context c [concat (app ?l1 ?l2)] => rewrite concat_app
+    (* idck_app, idty_app *)
+    | H: context c [idty (?l1 ++ ?l2)] |- _ => rewrite idty_app in H
+    | H: context c [idck (?l1 ++ ?l2)] |- _ => rewrite idck_app in H
+    (* app_nil_r *)
+    | H: context c [app ?l nil] |- _ => rewrite app_nil_r in H
+    | |- context c [app ?l nil] => rewrite app_nil_r
+    (* app_assoc *)
+    | H: context c [app (app ?l1 ?l2) ?l3] |- _ => rewrite <- app_assoc in H
+    | |- context c [app (app ?l1 ?l2) ?l3] => rewrite <- app_assoc
+    end.
+
+  (** ** Length of normalized expression *)
+
+  Ltac rewrite_Forall_forall :=
+    match goal with
+    | H : Forall _ _ |- _ =>
+      rewrite Forall_forall in H
+    | H : Forall2 _ _ _ |- _ =>
+      rewrite Forall2_forall2 in H; destruct H
+    | H : Forall3 _ _ _ _ |- _ =>
+      rewrite Forall3_forall3 in H; destruct H as [? [? ?]]
+    | |- Forall _ _ =>
+      rewrite Forall_forall; intros; subst
+    | |- Forall2 _ _ _ =>
+      rewrite Forall2_forall2; repeat split; auto; intros; subst
+    | |- Forall3 _ _ _ _ =>
+      rewrite Forall3_forall3; repeat split; auto; intros; subst
+    end.
+
+  Ltac subst_length :=
+    match goal with
+    | H: length ?x1 = length ?x2 |- context l [length ?x1] =>
+      setoid_rewrite H
+    | H: length ?x1 = length ?x2, H1: context l [length ?x1] |- _ =>
+      setoid_rewrite H in H1
+    | H: ?x1 = ?x2 |- context l [length ?x1] =>
+      setoid_rewrite H
+    | H: ?x1 = ?x2, H1: context l [length ?x1] |- _ =>
+      setoid_rewrite H in H1
+    end.
+
+  Ltac simpl_length :=
+    repeat subst_length;
+    (match goal with
+     | H : context c [typesof _] |- _ =>
+       rewrite typesof_annots in H
+     | H : context c [clocksof _] |- _ =>
+       rewrite clocksof_annots in H
+     | H : _ < Nat.min _ _ |- _ =>
+       setoid_rewrite Nat.min_glb_lt_iff in H; destruct H
+     | H : context c [Nat.min ?x1 ?x1] |- _ =>
+       repeat setoid_rewrite PeanoNat.Nat.min_id in H
+     | H : context c [length (combine _ _)] |- _ =>
+       setoid_rewrite combine_length in H
+     | H : context c [length (map ?l1 ?l2)] |- _ =>
+       setoid_rewrite map_length in H
+     | |- _ < Nat.min _ _ =>
+       apply Nat.min_glb_lt
+     | |- context c [Nat.min ?x1 ?x1] =>
+       setoid_rewrite PeanoNat.Nat.min_id
+     | |- context c [length (combine _ _)] =>
+       setoid_rewrite combine_length
+     | |- context c [length (map _ _)] =>
+       setoid_rewrite map_length
+     | |- context c [typesof _] =>
+       rewrite typesof_annots
+     | |- context c [clocksof _] =>
+       rewrite clocksof_annots
+     | _ => idtac
+    end).
+
+  Ltac solve_length :=
+    repeat simpl_length; auto; try congruence.
+
+  Ltac simpl_nth :=
+    match goal with
+    | H : In ?x _ |- _ =>
+      apply In_nth with (d:=x) in H; destruct H as [? [? ?]]
+    | H : context c [nth _ (combine _ _) (?x1, ?x2)] |- _ =>
+      rewrite (combine_nth _ _ _ x1 x2) in H; [inv H|clear H;try solve_length]
+    | H : context c [nth _ (map _ _) _] |- _ =>
+      erewrite map_nth' in H; [|clear H; try solve_length]
+    | |- context c [nth _ (map _ _) _] =>
+      erewrite map_nth'; [| try solve_length]
+    end.
+
+  Fact map_bind2_length : forall is_control es es' eqs' st st',
+      Forall2 (fun e es' => forall eqs' st st',
+                   normalize_exp is_control e st = (es', eqs', st') ->
+                   length es' = numstreams e) es es' ->
+    map_bind2 (normalize_exp is_control) es st = (es', eqs', st') ->
+    length (concat es') = length (annots es).
+  Proof.
+    intros is_control es es' eqs' st st' Hf Hmap.
+    apply map_bind2_values in Hmap.
+    repeat simpl_list.
+    apply concat_length_eq.
+    rewrite Forall2_map_2, Forall2_swap_args.
+    eapply Forall3_ignore3, Forall2_Forall2 in Hmap; [| eapply Hf]. clear Hf.
+    eapply Forall2_impl_In; eauto.
+    intros ? ? _ _ [H1 [? [? [? H2]]]]. rewrite length_annot_numstreams; eauto.
+  Qed.
+
+  Local Hint Resolve nth_In.
+  Fact normalize_exp_length : forall G e is_control es' eqs' st st',
+      wl_exp G e ->
+      normalize_exp is_control e st = (es', eqs', st') ->
+      length es' = numstreams e.
+  Proof with eauto.
+    induction e using exp_ind2; intros is_control es' eqs' st st' Hwl Hnorm;
+      simpl in *; inv Hwl; repeat inv_bind; auto.
+    - (* fby *)
+      simpl in *. rewrite map_length.
+      apply idents_for_anns_length in H3...
+    - (* when *)
+      unfold normalize_when. rewrite map_length.
+      eapply map_bind2_length in H0.
+      + solve_length.
+      + eapply map_bind2_values in H0.
+        repeat rewrite_Forall_forall...
+    - (* merge *)
+      destruct is_control; repeat inv_bind; unfold normalize_merge.
+      + apply map_bind2_length in H1; [| eapply map_bind2_values in H1; repeat rewrite_Forall_forall; eauto].
+        apply map_bind2_length in H2; [| eapply map_bind2_values in H2; repeat rewrite_Forall_forall; eauto].
+        solve_length.
+      + apply idents_for_anns_length in H3. solve_length.
+    - (* ite *)
+      destruct is_control; repeat inv_bind; unfold normalize_ite.
+      + apply map_bind2_length in H2; [| eapply map_bind2_values in H2; repeat rewrite_Forall_forall; eauto].
+        apply map_bind2_length in H3; [| eapply map_bind2_values in H3; repeat rewrite_Forall_forall; eauto].
+        solve_length.
+      + apply idents_for_anns_length in H4. solve_length.
+    - (* app *)
+      apply idents_for_anns'_length in H2.
+      solve_length.
+    - (* app (reset) *)
+      apply idents_for_anns'_length in H3.
+      solve_length.
+  Qed.
+  Hint Resolve normalize_exp_length.
+
+  Corollary map_bind2_normalize_exp_length : forall G is_control es es' eqs' st st',
+      Forall (wl_exp G) es ->
+      map_bind2 (normalize_exp is_control) es st = (es', eqs', st') ->
+      length (concat es') = length (annots es).
+  Proof.
+    intros G is_control es es' eqs' st st' Hf Hmap.
+    eapply map_bind2_length; eauto.
+    eapply map_bind2_values in Hmap.
+    repeat rewrite_Forall_forall.
+    eapply normalize_exp_length; eauto.
+  Qed.
+  Hint Resolve map_bind2_normalize_exp_length.
+
+  Corollary normalize_exps_length : forall G es es' eqs' st st',
+      Forall (wl_exp G) es ->
+      normalize_exps es st = (es', eqs', st') ->
+      length es' = length (annots es).
+  Proof.
+    intros G es es' eqs' st st' Hwt Hnorm.
+    unfold normalize_exps in Hnorm.
+    repeat inv_bind.
+    eapply map_bind2_normalize_exp_length; eauto.
+  Qed.
+  Hint Resolve normalize_exps_length.
+
+  Fact normalize_fby_length : forall e0s es anns,
+      length e0s = length anns ->
+      length es = length anns ->
+      length (normalize_fby e0s es anns) = length anns.
+  Proof.
+    intros * Hl1 Hl2.
+    unfold normalize_fby. solve_length.
+  Qed.
+
+  Fact normalize_merge_length : forall ckid ets efs tys nck,
+    length ets = length tys ->
+    length efs = length tys ->
+    length (normalize_merge ckid ets efs tys nck) = length tys.
+  Proof.
+    intros * Hl1 Hl2.
+    unfold normalize_merge. solve_length.
+  Qed.
+
+  Fact normalize_ite_length : forall e ets efs tys nck,
+    length ets = length tys ->
+    length efs = length tys ->
+    length (normalize_ite e ets efs tys nck) = length tys.
+  Proof.
+    intros * Hl1 Hl2.
+    unfold normalize_ite. solve_length.
+  Qed.
+
+  Fact normalize_rhs_length : forall G e es' eqs' st st',
+      wl_exp G e ->
+      normalize_rhs e st = (es', eqs', st') ->
+      (length es' = 1 \/ length es' = numstreams e).
+  Proof.
+    intros * Hwt Hnorm;
+      destruct e; unfold normalize_rhs in Hnorm;
+        try (solve [right; eapply normalize_exp_length; eauto]);
+        try (destruct o); repeat inv_bind; auto.
+    (* keep_fby = true *)
+    right. inv Hwt.
+    eapply normalize_fby_length; eauto.
+    - eapply normalize_exps_length in H; eauto. congruence.
+    - eapply normalize_exps_length in H0; eauto. congruence.
+  Qed.
+  Hint Resolve normalize_rhs_length.
+
+  Fact normalize_exp_numstreams : forall e is_control es' eqs' st st',
+      normalize_exp is_control e st = (es', eqs', st') ->
+      Forall (fun e => numstreams e = 1) es'.
+  Proof.
+    intros e is_control es' eqs' st st' Hnorm.
+    induction e; simpl in Hnorm; repeat inv_bind; repeat constructor.
+    2: destruct l0.
+    3,4: destruct l1.
+    3,4: destruct is_control.
+    1,2,3,4,5,6,7:(repeat inv_bind; unfold normalize_when, normalize_merge, normalize_ite;
+                   rewrite Forall_forall; intros ? Hin;
+                   repeat simpl_In; reflexivity).
+  Qed.
+
+  Corollary map_bind2_normalize_exp_numstreams : forall es is_control es' eqs' st st',
+      map_bind2 (normalize_exp is_control) es st = (es', eqs', st') ->
+      Forall (fun e => numstreams e = 1) (concat es').
+  Proof.
+    intros es is_control es' eqs' st st' Hmap.
+    apply map_bind2_values in Hmap.
+    induction Hmap; simpl.
+    - constructor.
+    - apply Forall_app; split; auto.
+      destruct H as [? [? H]].
+      eapply normalize_exp_numstreams; eauto.
+  Qed.
+
+  Corollary normalize_exps_numstreams : forall es es' eqs' st st',
+      normalize_exps es st = (es', eqs', st') ->
+      Forall (fun e => numstreams e = 1) es'.
+  Proof.
+    intros es es' eqs' st st' Hnorm.
+    unfold normalize_exps in Hnorm. repeat inv_bind.
+    eapply map_bind2_normalize_exp_numstreams. eauto.
+  Qed.
+
+  (** ** Preservation of annotations *)
+
+  Definition without_names (vars : list ann) : list (Op.type * clock) :=
+    List.map (fun '(ty, (cl, _)) => (ty, cl)) vars.
+
+  Fact without_names_length : forall anns,
+      length (without_names anns) = length anns.
+  Proof.
+    intros. unfold without_names. apply map_length.
+  Qed.
+
+  Fact idents_for_anns_annots : forall anns ids st st',
+      idents_for_anns anns st = (ids, st') ->
+      annots (map (fun '(x, a) => Evar x a) ids) = anns.
+  Proof.
+    intros.
+    eapply idents_for_anns_values in H; subst.
+    induction ids; simpl; auto.
+    destruct a; simpl. f_equal; auto.
+  Qed.
+
+  Fact idents_for_anns'_annots : forall anns ids st st',
+      idents_for_anns' anns st = (ids, st') ->
+      annots (map (fun '(x, a) => Evar x a) ids) = anns.
+  Proof.
+    intros.
+    eapply idents_for_anns'_values in H; subst.
+    induction ids; simpl; auto.
+    destruct a; simpl. f_equal; auto.
+  Qed.
+
+  Fact normalize_merge_annot : forall ckid ets efs tys ck,
+      length ets = length tys ->
+      length efs = length tys ->
+      Forall2 (fun ty e => annot e = [(ty, ck)]) tys (normalize_merge ckid ets efs tys ck).
+  Proof.
+    intros * Hlen1 Hlen2. unfold normalize_merge. rewrite Forall2_map_2.
+    revert ets efs Hlen1 Hlen2.
+    induction tys; intros; destruct ets, efs; simpl in *; try congruence;
+      constructor; auto.
+  Qed.
+
+  Fact normalize_ite_annot : forall e ets efs tys ck,
+      length ets = length tys ->
+      length efs = length tys ->
+      Forall2 (fun ty e => annot e = [(ty, ck)]) tys (normalize_ite e ets efs tys ck).
+  Proof.
+    intros * Hlen1 Hlen2. unfold normalize_ite. rewrite Forall2_map_2.
+    revert ets efs Hlen1 Hlen2.
+    induction tys; intros; destruct ets, efs; simpl in *; try congruence;
+      constructor; auto.
+  Qed.
+
+  Fact normalize_exp_annot : forall G e is_control es' eqs' st st',
+      wl_exp G e ->
+      normalize_exp is_control e st = (es', eqs', st')  ->
+      annots es' = annot e.
+  Proof with eauto.
+    destruct e; intros is_control es' eqs' st st' Hwl Hnorm;
+      (* specialize (normalize_exp_length _ _ _ es' eqs' st st' Hwl Hnorm) as Hlength; *)
+        inv Hwl; repeat inv_bind...
+    - (* fby *) apply idents_for_anns_annots in H1...
+    - (* when *)
+      assert (length (concat x0) = length (annots l)) as Hlen by eauto.
+      repeat simpl_list.
+      rewrite H5 in Hlen.
+      remember (concat x0) as l0.
+      clear x0 H H2 H5 Heql0. revert l0 Hlen.
+      induction tys; intros l0 Hlen; destruct l0; simpl in *; try congruence.
+      destruct nck. f_equal; auto.
+    - (* merge *)
+      destruct is_control; repeat inv_bind.
+      + assert (length (concat x2) = length (annots l)) as Hlen1 by eauto; rewrite H6 in Hlen1.
+        assert (length (concat x5) = length (annots l0)) as Hlen2 by eauto; rewrite H7 in Hlen2.
+        repeat simpl_list.
+        remember (concat x2) as l1. remember (concat x5) as l2.
+        clear x2 x5 H H0 H4 H5 H6 H7 Heql1 Heql2. revert l1 l2 Hlen1 Hlen2.
+        induction tys; intros l1 l2 Hlen1 Hlen2; destruct l1; destruct l2; simpl in *; try congruence.
+        destruct nck. f_equal; auto.
+      + apply idents_for_anns_annots in H1...
+    - (* ite *)
+      destruct is_control; repeat inv_bind.
+      + assert (length (concat x5) = length (annots l)) as Hlen1 by eauto; rewrite H8 in Hlen1.
+        assert (length (concat x8) = length (annots l0)) as Hlen2 by eauto; rewrite H9 in Hlen2.
+        repeat simpl_list.
+        remember (concat x5) as l1. remember (concat x8) as l2.
+        clear x5 x8 H0 H1 H8 H9 Heql1 Heql2. revert l1 l2 Hlen1 Hlen2.
+        induction tys; intros l1 l2 Hlen1 Hlen2; destruct l1; destruct l2; simpl in *; try congruence.
+        destruct nck. f_equal; auto.
+      + apply idents_for_anns_annots in H2...
+    - (* app *) apply idents_for_anns'_annots in H0...
+    - (* app (reset) *) apply idents_for_anns'_annots in H1...
+  Qed.
+
+  Corollary normalize_exp_annot_length : forall G e is_control es' eqs' st st',
+      wl_exp G e ->
+      normalize_exp is_control e st = (es', eqs', st')  ->
+      length (annots es') = length (annot e).
+  Proof with eauto.
+    intros.
+    eapply normalize_exp_annot in H0; eauto.
+    congruence.
+  Qed.
+
+  Fact map_bind2_normalize_exp_annots': forall G is_control es es' eqs' st st',
+      Forall (wl_exp G) es ->
+      map_bind2 (normalize_exp is_control) es st = (es', eqs', st') ->
+      Forall2 (fun es' e => annots es' = annot e) es' es.
+  Proof.
+    intros G is_control es es' eqs' st st' Hf Hmap.
+    apply map_bind2_values in Hmap.
+    induction Hmap.
+    - constructor.
+    - destruct H as [? [? Hnorm]]. inv Hf.
+      constructor; eauto.
+      eapply normalize_exp_annot; eauto.
+  Qed.
+
+  Corollary map_bind2_normalize_exp_annots'' : forall G is_control es es' eqs' st st',
+      Forall (wl_exp G) es ->
+      map_bind2 (normalize_exp is_control) es st = (es', eqs', st') ->
+      Forall2 (fun e ann => annot e = [ann]) (concat es') (annots es).
+  Proof.
+    intros * Hwl Hmap.
+    assert (Forall (fun e => numstreams e = 1) (concat es')) as Hnumstreams.
+    { eapply map_bind2_normalize_exp_numstreams in Hmap; eauto. }
+    eapply map_bind2_normalize_exp_annots' in Hmap; eauto.
+    unfold annots; rewrite flat_map_concat_map.
+    apply Forall2_concat. rewrite Forall2_map_2.
+    eapply Forall2_impl_In; eauto. clear Hmap. intros; simpl in *.
+    rewrite <- H1, <- (concat_map_singl1 a) at 1.
+    unfold annots; rewrite flat_map_concat_map.
+    apply Forall2_concat. rewrite Forall2_map_1, Forall2_map_2.
+    apply Forall2_same, Forall_forall. intros.
+    assert (In x (concat es')) as HIn by eauto using in_concat'.
+    eapply Forall_forall in HIn; eauto; simpl in HIn.
+    rewrite <- length_annot_numstreams in HIn. singleton_length.
+    repeat constructor; auto.
+  Qed.
+
+  Corollary map_bind2_normalize_exp_annots_length' :
+    forall G is_control es es' eqs' st st',
+      Forall (wl_exp G) es ->
+      map_bind2 (normalize_exp is_control) es st = (es', eqs', st') ->
+      Forall2 (fun es' e => length (annots es') = length (annot e)) es' es.
+  Proof.
+    intros G is_control es es' eqs' st st' Hf Hmap.
+    eapply map_bind2_normalize_exp_annots' in Hmap; eauto.
+    induction Hmap; inv Hf; constructor; eauto.
+    congruence.
+  Qed.
+
+  Fact map_bind2_normalize_exp_annots :
+    forall G is_control es es' eqs' st st',
+      Forall (wl_exp G) es ->
+      map_bind2 (normalize_exp is_control) es st = (es', eqs', st') ->
+      annots (concat es') = annots es.
+  Proof.
+    intros G is_control es es' a2s st st' Hwl Hmap.
+    eapply map_bind2_normalize_exp_annots' in Hmap; eauto.
+    induction Hmap; simpl; auto.
+    inv Hwl.
+    repeat simpl_list.
+    f_equal; auto.
+  Qed.
+
+  Fact map_bind2_normalize_exp_annots_length :
+    forall G is_control es es' eqs' st st',
+      Forall (wl_exp G) es ->
+      map_bind2 (normalize_exp is_control) es st = (es', eqs', st') ->
+      length (annots (concat es')) = length (annots es).
+  Proof.
+    intros G is_control es es' a2s st st' Hwl Hmap.
+    eapply map_bind2_normalize_exp_annots in Hmap; eauto.
+    congruence.
+  Qed.
+
+  Fact normalize_exps_annots : forall G es es' eqs' st st',
+      Forall (wl_exp G) es ->
+      normalize_exps es st = (es', eqs', st') ->
+      annots es' = annots es.
+  Proof.
+    intros G es es' eqs' st st' Hwt Hnorm.
+    unfold normalize_exps in Hnorm; repeat inv_bind.
+    eapply map_bind2_normalize_exp_annots in H; eauto.
+  Qed.
+
+  Corollary normalize_exps_annots_length : forall G es es' eqs' st st',
+      Forall (wl_exp G) es ->
+      normalize_exps es st = (es', eqs', st') ->
+      length (annots es') = length (annots es).
+  Proof.
+    intros G es es' eqs' st st' Hwt Hnorm.
+    eapply normalize_exps_annots in Hnorm; eauto.
+    congruence.
+  Qed.
+
+  Fact normalize_fby_annot : forall anns e0s es,
+      length e0s = length anns ->
+      length es = length anns ->
+      annots (normalize_fby e0s es anns) = anns.
+  Proof.
+    induction anns; intros * Hl1 Hl2;
+      destruct e0s; destruct es; simpl in *; try congruence; auto.
+    f_equal. eauto.
+  Qed.
+
+  Fact normalize_rhs_annot : forall G e es' eqs' st st',
+      wl_exp G e ->
+      normalize_rhs e st = (es', eqs', st') ->
+      annots es' = annot e.
+  Proof.
+    intros * Hwt Hnorm.
+    destruct e; unfold normalize_rhs in Hnorm;
+      try (solve [eapply normalize_exp_annot in Hnorm; eauto]).
+    - (* fby *)
+      repeat inv_bind. inv Hwt.
+      eapply normalize_fby_annot; eauto.
+      + eapply normalize_exps_length in H; eauto. congruence.
+      + eapply normalize_exps_length in H0; eauto. congruence.
+    - (* app *)
+      destruct o; repeat inv_bind; simpl; rewrite app_nil_r; reflexivity.
+  Qed.
+
+  Corollary normalize_rhs_annot_length : forall G e es' eqs' st st',
+      wl_exp G e ->
+      normalize_rhs e st = (es', eqs', st') ->
+      length (annots es') = length (annot e).
+  Proof.
+    intros * Hwt Hnorm.
+    eapply normalize_rhs_annot in Hnorm; eauto.
+    congruence.
+  Qed.
+
+  Fact normalize_rhss_annots : forall G es es' eqs' st st',
+      Forall (wl_exp G) es ->
+      normalize_rhss es st = (es', eqs', st') ->
+      annots es' = annots es.
+  Proof.
+    intros * Hf Hnorm.
+    unfold normalize_rhss in Hnorm. repeat inv_bind.
+    apply map_bind2_values in H.
+    induction H; simpl in *.
+    - reflexivity.
+    - inv Hf.
+      destruct H as [? [? H]]. eapply normalize_rhs_annot in H; eauto.
+      repeat simpl_list.
+      f_equal; auto.
+  Qed.
+
+  Corollary normalize_rhss_annots_length : forall G es es' eqs' st st',
+      Forall (wl_exp G) es ->
+      normalize_rhss es st = (es', eqs', st') ->
+      length (annots es') = length (annots es).
+  Proof.
+    intros G es es' eqs' st st' Hf Hnorm.
+    eapply normalize_rhss_annots in Hnorm; eauto.
+    congruence.
+  Qed.
+
+  (** ** Propagation of the variable permutation property *)
+
+  Fact idents_for_anns_vars_perm : forall anns ids st st',
+      idents_for_anns anns st = (ids, st') ->
+      Permutation ((map fst ids)++(st_ids st)) (st_ids st').
+  Proof.
+    induction anns; intros ids st st' Hidents; simpl in Hidents; repeat inv_bind.
+    - reflexivity.
+    - destruct a as [ty [cl name]]. repeat inv_bind.
+      apply fresh_ident_vars_perm in H.
+      apply IHanns in H0.
+      etransitivity. 2: eapply H0.
+      etransitivity. eapply Permutation_middle.
+      apply Permutation_app_head. assumption.
+  Qed.
+
+  Fact idents_for_anns'_vars_perm : forall anns ids st st',
+      idents_for_anns' anns st = (ids, st') ->
+      Permutation ((map fst ids)++(st_ids st)) (st_ids st').
+  Proof.
+    induction anns; intros ids st st' Hidents; simpl in Hidents; repeat inv_bind.
+    - reflexivity.
+    - destruct a as [ty [cl [name|]]]; repeat inv_bind.
+      1: (destruct x; apply reuse_ident_vars_perm in H).
+      2: apply fresh_ident_vars_perm in H.
+      1,2: (apply IHanns in H0;
+            etransitivity; [| eapply H0];
+            etransitivity; [eapply Permutation_middle|];
+            apply Permutation_app_head; auto).
+  Qed.
+
+  Fact map_bind2_vars_perm {A B} : forall (k : A -> FreshAnn (B * list equation)) es es' eqs' st st',
+      map_bind2 k es st = (es', eqs', st') ->
+      Forall (fun e => forall es' eqs' st st',
+                  k e st = (es', eqs', st') ->
+                  Permutation ((vars_defined eqs')++(st_ids st)) (st_ids st')) es ->
+      Permutation ((vars_defined (concat eqs'))++(st_ids st)) (st_ids st').
+  Proof.
+    induction es; intros es' eqs' st st' Hmap Hf;
+      repeat inv_bind.
+    - reflexivity.
+    - inv Hf.
+      specialize (IHes _ _ _ _ H0 H4).
+      specialize (H3 _ _ _ _ H).
+      etransitivity. 2: apply IHes.
+      repeat simpl_list.
+      rewrite Permutation_swap.
+      apply Permutation_app_head. assumption.
+  Qed.
+
+  Fact normalize_reset_vars_perm : forall e e' eqs' st st',
+      normalize_reset e st = ((e', eqs'), st') ->
+      Permutation ((vars_defined eqs')++(st_ids st)) (st_ids st').
+  Proof.
+    intros e e' eqs' st st' Hnorm.
+    destruct (normalize_reset_spec e) as [[v [ann [Hv Hspec]]]| Hspec];
+      subst; rewrite Hspec in Hnorm; clear Hspec.
+    - repeat inv_bind. reflexivity.
+    - destruct (hd _ _) as [ty [cl _]]. repeat inv_bind.
+      eapply fresh_ident_vars_perm; eauto.
+  Qed.
+
+  Fact normalize_exp_vars_perm : forall G e is_control es' eqs' st st',
+      wl_exp G e ->
+      normalize_exp is_control e st = ((es', eqs'), st') ->
+      Permutation ((vars_defined eqs')++(st_ids st)) (st_ids st')(* ++(fresh_in e) *).
+  Proof with eauto.
+    induction e using exp_ind2; intros is_control e' eqs' st st' Hwt Hnorm;
+      simpl in Hnorm; inv Hwt.
+    - (* const *)
+      repeat inv_bind...
+    - (* var *)
+      repeat inv_bind...
+    - (* unop *)
+      repeat inv_bind...
+    - (* binop *)
+      repeat inv_bind.
+      repeat simpl_list.
+      apply IHe1 in H...
+      apply IHe2 in H0...
+      etransitivity. 2: eauto. repeat simpl_list.
+      rewrite Permutation_swap.
+      apply Permutation_app_head...
+    - (* fby *)
+      repeat inv_bind.
+      remember (normalize_fby _ _ _) as fby.
+      assert (length x5 = length fby) as Hlen.
+      { eapply map_bind2_normalize_exp_length in H1...
+        eapply map_bind2_normalize_exp_length in H2...
+        apply idents_for_anns_length in H3...
+        rewrite Heqfby, normalize_fby_length; solve_length.
+      }
+      apply map_bind2_vars_perm in H1. 2:solve_forall.
+      apply map_bind2_vars_perm in H2. 2:solve_forall.
+      apply idents_for_anns_vars_perm in H3.
+      repeat simpl_list.
+      etransitivity. 2:apply H3.
+      replace (map (fun x => fst (let '(x0, _, fby) := x in ([x0], [fby]))) (combine x5 _)) with (map (fun x => [fst x]) x5).
+      2: { clear - Hlen. revert fby Hlen.
+           induction x5; intros; destruct fby; simpl in *; try congruence.
+           destruct a. f_equal; eauto. }
+      repeat rewrite concat_app.
+      replace (concat (map (fun x => [fst x]) x5)) with (map fst x5).
+      2: { clear. induction x5; simpl; f_equal; auto. }
+      repeat rewrite <- app_assoc. apply Permutation_app_head.
+      etransitivity. 2: eauto.
+      rewrite Permutation_swap. apply Permutation_app_head; auto.
+    - (* when *)
+      repeat inv_bind.
+      eapply map_bind2_vars_perm...
+      rewrite Forall_forall in *. intros...
+    - (* merge *)
+      destruct is_control; repeat inv_bind.
+      + apply map_bind2_vars_perm in H1. 2: (rewrite Forall_forall in *; eauto).
+        apply map_bind2_vars_perm in H2. 2: (rewrite Forall_forall in *; eauto).
+        etransitivity. 2: apply H2.
+        repeat simpl_list.
+        rewrite Permutation_swap. apply Permutation_app_head.
+        assumption.
+      + repeat simpl_list.
+        rewrite combine_map_fst'.
+        2: {
+          repeat rewrite map_length. repeat rewrite combine_length.
+          repeat rewrite typesof_annots in *.
+          assert (length (concat x3) = length (annots ets)) as Hlen3 by eauto.
+          assert (length (concat x7) = length (annots efs)) as Hlen7 by eauto.
+          apply idents_for_anns_length in H3.
+          repeat simpl_list. solve_length. }
+        apply map_bind2_vars_perm in H1. 2: (repeat rewrite_Forall_forall; eauto).
+        apply map_bind2_vars_perm in H2. 2: (repeat rewrite_Forall_forall; eauto).
+        apply idents_for_anns_vars_perm in H3.
+        etransitivity. 2: eauto.
+        replace (concat (map (fun '(id, _) => [id]) x6)) with (map fst x6).
+        2: { clear H3. induction x6; try destruct a; simpl; f_equal; auto. }
+        repeat rewrite <- app_assoc. apply Permutation_app_head.
+        etransitivity. 2: eauto.
+        repeat simpl_list.
+        rewrite Permutation_swap. apply Permutation_app_head.
+        assumption.
+    - (* ite *)
+      destruct is_control; repeat inv_bind.
+      + apply map_bind2_vars_perm in H2. 2: (rewrite Forall_forall in *; eauto).
+        apply map_bind2_vars_perm in H3. 2: (rewrite Forall_forall in *; eauto).
+        apply IHe in H1; eauto.
+        etransitivity. 2: eauto.
+        unfold vars_defined in *; repeat rewrite <- flat_map_app.
+        rewrite <- app_assoc. rewrite Permutation_swap.
+        rewrite <- app_assoc. rewrite Permutation_swap. apply Permutation_app_head.
+        etransitivity. 2: eauto.
+        apply Permutation_app_head.
+        assumption.
+      + repeat simpl_list.
+        rewrite combine_map_fst'.
+        2: {
+          repeat rewrite map_length. repeat rewrite combine_length.
+          repeat rewrite typesof_annots in *.
+          assert (length (concat x5) = length (annots ets)) as Hlen3 by eauto.
+          assert (length (concat x9) = length (annots efs)) as Hlen7 by eauto.
+          apply idents_for_anns_length in H4.
+          repeat simpl_list. solve_length. }
+        apply map_bind2_vars_perm in H2. 2: (repeat rewrite_Forall_forall; eauto).
+        apply map_bind2_vars_perm in H3. 2: (repeat rewrite_Forall_forall; eauto).
+        apply idents_for_anns_vars_perm in H4.
+        apply IHe in H1; eauto.
+        etransitivity. 2: eauto.
+        replace (concat (map (fun '(id, _) => [id]) x8)) with (map fst x8).
+        2: { clear H4. induction x8; try destruct a; simpl; f_equal; auto. }
+        repeat rewrite <- app_assoc. apply Permutation_app_head.
+        etransitivity. 2: eauto.
+        repeat simpl_list.
+        rewrite app_assoc. rewrite Permutation_swap. apply Permutation_app_head.
+        etransitivity. 2: eauto.
+        rewrite <- app_assoc. rewrite Permutation_swap. apply Permutation_app_head.
+        assumption.
+    - (* app *)
+      repeat inv_bind.
+      assert (length x1 = length a) as Hlen by eauto.
+      apply idents_for_anns'_vars_perm in H2.
+      apply map_bind2_vars_perm in H1. 2: (repeat rewrite_Forall_forall; eauto).
+      etransitivity. 2: apply H2.
+      rewrite <- app_assoc.
+      apply Permutation_app_head. rewrite app_nil_r. assumption.
+    - (* app (reset) *)
+      repeat inv_bind.
+      assert (length x5 = length a) as Hlen by eauto.
+      apply idents_for_anns'_vars_perm in H3.
+      apply map_bind2_vars_perm in H1. 2: (repeat rewrite_Forall_forall; eauto).
+      apply normalize_reset_vars_perm in H4.
+      apply H in H2; eauto.
+      etransitivity. 2: eauto.
+      repeat rewrite <- app_assoc.
+      apply Permutation_app_head.
+      repeat simpl_list.
+      etransitivity; [| eauto].
+      rewrite Permutation_app_comm, Permutation_swap, <- app_assoc.
+      apply Permutation_app_head.
+      etransitivity; [| eauto].
+      repeat simpl_list. apply Permutation_app_head.
+      rewrite Permutation_app_comm. assumption.
+  Qed.
+
+  Corollary normalize_exps_vars_perm : forall G es es' eqs' st st',
+      Forall (wl_exp G) es ->
+      normalize_exps es st = ((es', eqs'), st') ->
+      Permutation ((vars_defined eqs')++(st_ids st)) (st_ids st').
+  Proof with eauto.
+    intros G es es' eqs' st st' Hf Hnorm.
+    unfold normalize_exps in Hnorm.
+    repeat inv_bind.
+    eapply map_bind2_vars_perm...
+    repeat rewrite_Forall_forall.
+    eapply normalize_exp_vars_perm...
+  Qed.
+
+  Fact normalize_rhs_vars_perm : forall G e es' eqs' st st',
+      wl_exp G e ->
+      normalize_rhs e st = ((es', eqs'), st') ->
+      Permutation ((vars_defined eqs')++(st_ids st)) (st_ids st').
+  Proof with eauto.
+    intros * Hwt Hnorm.
+    destruct e; unfold normalize_rhs in Hnorm;
+      try (solve [eapply normalize_exp_vars_perm; eauto]); inv Hwt; repeat inv_bind.
+    - (* fby *)
+      repeat inv_bind.
+      eapply normalize_exps_vars_perm in H...
+      eapply normalize_exps_vars_perm in H0...
+      etransitivity. 2: eauto.
+      repeat simpl_list.
+      rewrite Permutation_swap. apply Permutation_app_head; auto.
+    - (* app *)
+      eapply normalize_exps_vars_perm in H; eauto.
+      rewrite app_nil_r; eauto.
+    - (* app (reset) *)
+      eapply normalize_exps_vars_perm in H; eauto.
+      eapply normalize_exp_vars_perm in H0; eauto.
+      eapply normalize_reset_vars_perm in H1.
+      etransitivity. 2: eauto.
+      repeat simpl_list.
+      rewrite Permutation_app_comm, Permutation_swap, <- app_assoc, <- app_assoc.
+      apply Permutation_app_head.
+      etransitivity. 2: eauto.
+      apply Permutation_app_head.
+      rewrite Permutation_app_comm.
+      assumption.
+  Qed.
+
+  Corollary normalize_rhss_vars_perm : forall G es es' eqs' st st',
+      Forall (wl_exp G) es ->
+      normalize_rhss es st = ((es', eqs'), st') ->
+      Permutation ((vars_defined eqs')++(st_ids st)) (st_ids st').
+  Proof.
+    intros * Hf Hnorm.
+    unfold normalize_rhss in Hnorm.
+    repeat inv_bind.
+    eapply map_bind2_vars_perm in H; eauto.
+    repeat rewrite_Forall_forall.
+    eapply normalize_rhs_vars_perm; eauto.
+  Qed.
+
+  Fact split_equation_vars_defined : forall xs es,
+      length xs = length (annots es) ->
+      vars_defined (split_equation (xs, es)) = vars_defined [(xs, es)].
+  Proof.
+    intros xs es; revert xs.
+    induction es; intros xs Hwt; inv Hwt; simpl in *.
+    - destruct xs; simpl in *; congruence.
+    - specialize (IHes (skipn (numstreams a) xs)).
+      rewrite IHes.
+      + repeat rewrite app_nil_r. apply firstn_skipn.
+      + rewrite app_length in H0.
+        rewrite length_annot_numstreams in H0.
+        rewrite skipn_length. omega.
+  Qed.
+
+  Corollary split_equations_vars_defined : forall eqs,
+      Forall (fun '(xs, es) => length xs = length (annots es)) eqs ->
+      vars_defined (flat_map split_equation eqs) = vars_defined eqs.
+  Proof.
+    induction eqs; intro Hf; simpl in *; inv Hf.
+    - reflexivity.
+    - destruct a as [xs es]; simpl in H1.
+      specialize (split_equation_vars_defined _ _ H1) as Heq.
+      repeat simpl_list.
+      f_equal; simpl in *; auto.
+  Qed.
+
+  Fact untuple_equation_vars_perm : forall G eq eqs' st st',
+      wl_equation G eq ->
+      untuple_equation eq st = (eqs', st') ->
+      Permutation ((vars_defined eqs')++(st_ids st)) ((vars_defined [eq])++(st_ids st')).
+  Proof.
+    intros * Hwt Hnorm.
+    destruct eq; simpl in *.
+    repeat inv_bind. destruct Hwt as [Hwt Hl].
+    specialize (normalize_rhss_vars_perm _ _ _ _ _ _ Hwt H) as Hperm1.
+    rewrite app_nil_r.
+    assert (vars_defined (flat_map split_equation [(l, x)]) = vars_defined [(l, x)]) as Hxl.
+    { apply split_equations_vars_defined.
+      repeat constructor.
+      eapply normalize_rhss_annots_length in H; eauto. congruence. }
+    repeat simpl_list.
+    apply Permutation_app; auto.
+    rewrite <- Hxl at 2. reflexivity.
+  Qed.
+
+  Corollary untuple_equations_vars_perm : forall G eqs eqs' st st',
+      Forall (wl_equation G) eqs ->
+      untuple_equations eqs st = (eqs', st') ->
+      Permutation ((vars_defined eqs')++(st_ids st)) ((vars_defined eqs)++(st_ids st')).
+  Proof.
+    induction eqs; intros * Hf Hnorm; unfold untuple_equations in Hnorm; repeat inv_bind.
+    - reflexivity.
+    - inv Hf.
+      assert (untuple_equations eqs x1 = (concat x2, st')) as Hnorm'.
+      { unfold untuple_equations. repeat inv_bind. repeat eexists; eauto.
+        inv_bind; eauto. } eapply IHeqs in Hnorm'; eauto.
+      eapply untuple_equation_vars_perm in H; eauto; simpl in *.
+      repeat simpl_list.
+      rewrite Permutation_swap, H, Permutation_swap.
+      apply Permutation_app_head. assumption.
+  Qed.
+
+  (** ** Specification of an (almost) normalized node *)
+
+  Inductive normalized_lexp : exp -> Prop :=
+  | normalized_Econst : forall c, normalized_lexp (Econst c)
+  | normalized_Evar : forall x ty cl, normalized_lexp (Evar x (ty, cl))
+  | normalized_Eunop : forall op e1 ty cl,
+      normalized_lexp e1 ->
+      normalized_lexp (Eunop op e1 (ty, cl))
+  | normalized_Ebinop : forall op e1 e2 ty cl,
+      normalized_lexp e1 ->
+      normalized_lexp e2 ->
+      normalized_lexp (Ebinop op e1 e2 (ty, cl))
+  | normalized_Ewhen : forall e x b ty cl,
+      normalized_lexp e ->
+      normalized_lexp (Ewhen [e] x b ([ty], cl)).
+
+  Inductive normalized_cexp : exp -> Prop :=
+  | normalized_Emerge : forall x et ef ty cl,
+      normalized_cexp et ->
+      normalized_cexp ef ->
+      normalized_cexp (Emerge x [et] [ef] ([ty], cl))
+  | normalized_Eite : forall e et ef ty cl,
+      normalized_lexp e ->
+      normalized_cexp et ->
+      normalized_cexp ef ->
+      normalized_cexp (Eite e [et] [ef] ([ty], cl))
+  | normalized_lexp_cexp : forall e,
+      normalized_lexp e ->
+      normalized_cexp e.
+
+  Inductive untupled_equation : equation -> Prop :=
+  | untupled_eq_Eapp : forall xs f es lann,
+      Forall normalized_lexp es ->
+      untupled_equation (xs, [Eapp f es None lann])
+  | untupled_eq_Eapp_reset : forall xs f es x ty cl lann,
+      Forall normalized_lexp es ->
+      untupled_equation (xs, [Eapp f es (Some (Evar x (ty, cl))) lann])
+  | untupled_eq_Efby : forall x e0 e ann,
+      normalized_lexp e0 ->
+      normalized_lexp e ->
+      untupled_equation ([x], [Efby [e0] [e] [ann]])
+  | untupled_eq_cexp : forall x e,
+      normalized_cexp e ->
+      untupled_equation ([x], [e]).
+
+  Definition untupled_node (n : node) :=
+    Forall untupled_equation (n_eqs n).
+
+  Definition untupled_global (G : global) := Forall untupled_node G.
+
+  Hint Constructors normalized_lexp normalized_cexp untupled_equation.
+
+  (** A few initial properties *)
+
+  Fact normalized_lexp_numstreams : forall e,
+      normalized_lexp e ->
+      numstreams e = 1.
+  Proof.
+    induction e; intros Hnorm; inv Hnorm; reflexivity.
+  Qed.
+
+  Fact normalized_cexp_numstreams : forall e,
+      normalized_cexp e ->
+      numstreams e = 1.
+  Proof.
+    induction e; intros Hnorm; inv Hnorm;
+      try apply normalized_lexp_numstreams in H; auto.
+  Qed.
+
+  (** ** After normalization, equations and expressions are normalized *)
+
+  Fact normalized_lexp_hd_default : forall es,
+      Forall normalized_lexp es ->
+      normalized_lexp (hd_default es).
+  Proof.
+    intros es Hf.
+    destruct es; simpl.
+    - constructor.
+    - inv Hf; auto.
+  Qed.
+
+  Fact map_bind2_normalized_lexp' {A A2} :
+    forall (k : A -> FreshAnn ((list exp) * A2)) a es' a2s st st',
+      map_bind2 k a st = (es', a2s, st') ->
+      Forall (fun a => forall es' a2s st st',
+                  k a st = (es', a2s, st') ->
+                  Forall normalized_lexp es') a ->
+      Forall normalized_lexp (concat es').
+  Proof.
+    intros k a eqs' a2s st st' Hmap Hf.
+    apply map_bind2_values in Hmap.
+    induction Hmap; simpl in *.
+    - constructor.
+    - destruct H as [? [? H]]. inv Hf.
+      rewrite Forall_app.
+      split; eauto.
+  Qed.
+
+  Fact map_bind2_normalized_cexp' {A A2} :
+    forall (k : A -> FreshAnn ((list exp) * A2)) a es' a2s st st',
+      map_bind2 k a st = (es', a2s, st') ->
+      Forall (fun a => forall es' a2s st st',
+                  k a st = (es', a2s, st') ->
+                  Forall normalized_cexp es') a ->
+      Forall normalized_cexp (concat es').
+  Proof.
+    intros k a eqs' a2s st st' Hmap Hf.
+    apply map_bind2_values in Hmap.
+    induction Hmap; simpl in *.
+    - constructor.
+    - destruct H as [? [? H]]. inv Hf.
+      rewrite Forall_app.
+      split; eauto.
+  Qed.
+
+  Hint Resolve in_combine_l in_combine_r.
+  Hint Resolve normalized_lexp_hd_default.
+
+  Lemma normalize_exp_normalized_lexp : forall e es' eqs' st st',
+      normalize_exp false e st = (es', eqs', st') ->
+      Forall normalized_lexp es'.
+  Proof with eauto.
+    induction e using exp_ind2; intros es' eqs' st st' Hnorm;
+      repeat inv_bind; repeat constructor.
+    - (* var *)
+      destruct a...
+    - (* unop *)
+      destruct a...
+    - (* binop *)
+      destruct a. constructor...
+    - (* fby *)
+      simpl_forall.
+      repeat rewrite_Forall_forall.
+      repeat simpl_In. destruct a0...
+    - (* when *)
+      destruct a. repeat inv_bind. unfold normalize_when.
+      apply map_bind2_normalized_lexp' in H0...
+      repeat rewrite_Forall_forall.
+      repeat simpl_In...
+    - (* merge *)
+      destruct a. repeat inv_bind. unfold normalize_merge.
+      repeat rewrite_Forall_forall.
+      repeat simpl_In. destruct a...
+    - (* ite *)
+      destruct a. repeat inv_bind. unfold normalize_ite.
+      repeat rewrite_Forall_forall.
+      repeat simpl_In. destruct a...
+    - (* app *)
+      repeat rewrite_Forall_forall.
+      repeat simpl_In. destruct a0...
+  Qed.
+  Hint Resolve normalize_exp_normalized_lexp.
+
+  Corollary map_bind2_normalized_lexp : forall es es' eqs' st st',
+      map_bind2 (normalize_exp false) es st = (es', eqs', st') ->
+      Forall normalized_lexp (concat es').
+  Proof.
+    intros es es' eqs' st st' Hnorm.
+    eapply map_bind2_normalized_lexp' in Hnorm; auto.
+    solve_forall.
+  Qed.
+  Hint Resolve map_bind2_normalized_lexp.
+
+  Corollary normalize_exps_normalized_lexp: forall es es' eqs' st st',
+      normalize_exps es st = (es', eqs', st') ->
+      Forall normalized_lexp es'.
+  Proof.
+    intros es es' eqs' st st' Hnorm.
+    unfold normalize_exps in Hnorm. repeat inv_bind.
+    apply map_bind2_normalized_lexp in H; auto.
+  Qed.
+  Hint Resolve normalize_exps_normalized_lexp.
+
+  Fact normalize_reset_normalized_lexp : forall e e' eqs' st st',
+      normalize_reset e st = (e', eqs', st') ->
+      normalized_lexp e'.
+  Proof.
+    intros * Hnorm.
+    specialize (normalize_reset_spec e) as [[? [? [? Hspec]]]|Hspec]; subst;
+      rewrite Hspec in Hnorm; clear Hspec; repeat inv_bind.
+    - destruct x0. constructor.
+    - destruct hd as [? [? ?]] in Hnorm; repeat inv_bind.
+      constructor.
+  Qed.
+
+  Fact normalize_merge_normalized_cexp : forall x ets efs tys ck,
+      Forall normalized_cexp ets ->
+      Forall normalized_cexp efs ->
+      Forall normalized_cexp (normalize_merge x ets efs tys ck).
+  Proof.
+    intros. unfold normalize_merge.
+    repeat rewrite_Forall_forall. repeat simpl_In.
+    econstructor; eauto.
+  Qed.
+
+  Fact normalize_ite_normalized_cexp : forall e ets efs tys ck,
+      normalized_lexp e ->
+      Forall normalized_cexp ets ->
+      Forall normalized_cexp efs ->
+      Forall normalized_cexp (normalize_ite e ets efs tys ck).
+  Proof.
+    intros. unfold normalize_ite.
+    repeat rewrite_Forall_forall. repeat simpl_In.
+    econstructor; eauto.
+  Qed.
+
+  Lemma normalize_exp_normalized_cexp : forall e es' eqs' st st',
+      normalize_exp true e st = (es', eqs', st') ->
+      Forall normalized_cexp es'.
+  Proof with eauto.
+    induction e using exp_ind2; intros es' eqs' st st' Hnorm;
+      repeat inv_bind; repeat constructor.
+    - (* var *)
+      destruct a...
+    - (* unop *)
+      destruct a...
+    - (* binop *)
+      destruct a. constructor...
+    - (* fby *)
+      solve_forall.
+      repeat simpl_In. destruct a0...
+    - (* when *)
+      destruct a. repeat inv_bind. unfold normalize_when.
+      apply map_bind2_normalized_lexp in H0.
+      repeat rewrite_Forall_forall.
+      repeat simpl_In...
+    - (* merge *)
+      destruct a. repeat inv_bind.
+      eapply normalize_merge_normalized_cexp...
+      apply map_bind2_normalized_cexp' in H1; [|solve_forall]...
+      apply map_bind2_normalized_cexp' in H2; [|solve_forall]...
+    - (* ite *)
+      destruct a. repeat inv_bind.
+      eapply normalize_ite_normalized_cexp...
+      apply map_bind2_normalized_cexp' in H2; [|solve_forall]...
+      apply map_bind2_normalized_cexp' in H3; [|solve_forall]...
+    - (* app *)
+      solve_forall.
+      repeat simpl_In. destruct a0...
+  Qed.
+
+  Corollary map_bind2_normalized_cexp : forall es es' eqs' st st',
+      map_bind2 (normalize_exp true) es st = (es', eqs', st') ->
+      Forall normalized_cexp (concat es').
+  Proof.
+    intros. apply map_bind2_normalized_cexp' in H; auto.
+    solve_forall. apply normalize_exp_normalized_cexp in H1; auto.
+  Qed.
+
+  Fact map_bind2_untupled_eq {A A1} :
+    forall (k : A -> FreshAnn (A1 * (list equation))) a a1s eqs' st st',
+      map_bind2 k a st = (a1s, eqs', st') ->
+      Forall (fun a => forall a1s eqs' st st',
+                  k a st = (a1s, eqs', st') ->
+                  Forall untupled_equation eqs') a ->
+      Forall untupled_equation (concat eqs').
+  Proof.
+    induction a; intros * Hmap Hf;
+      repeat inv_bind.
+    - constructor.
+    - inv Hf. simpl.
+      rewrite Forall_app; eauto.
+  Qed.
+
+  Lemma normalize_exp_untupled_eq : forall e is_control es' eqs' st st',
+      normalize_exp is_control e st = (es', eqs', st') ->
+      Forall untupled_equation eqs'.
+  Proof with eauto.
+    induction e using exp_ind2; intros * Hnorm;
+      repeat inv_bind; repeat constructor; eauto.
+    - (* binop *)
+      apply Forall_app. split...
+    - (* fby *)
+      repeat rewrite Forall_app. repeat split.
+      + eapply map_bind2_normalized_lexp in H1.
+        eapply map_bind2_normalized_lexp in H2.
+        eapply Forall_forall; intros ? Hin.
+        unfold normalize_fby in Hin. repeat simpl_In.
+        constructor.
+        * eapply Forall_forall in H7...
+        * eapply Forall_forall in H5...
+      + eapply map_bind2_untupled_eq in H1... solve_forall.
+      + eapply map_bind2_untupled_eq in H2...
+        eapply map_bind2_st_follows in H1; solve_forall.
+    - (* when *)
+      destruct a. repeat inv_bind.
+      eapply map_bind2_untupled_eq in H0; eauto. solve_forall.
+    - (* merge *)
+      destruct a; destruct is_control; repeat inv_bind; unfold normalize_merge;
+        repeat rewrite Forall_app; repeat split.
+      1,2,4,5: (eapply map_bind2_untupled_eq; eauto; solve_forall).
+      rewrite Forall_forall; intros [? ?] Hin. rewrite map_map in Hin; simpl in Hin.
+      repeat simpl_In.
+      do 2 constructor.
+      + eapply map_bind2_normalized_cexp in H1.
+        rewrite Forall_forall in H1...
+      + eapply map_bind2_normalized_cexp in H2.
+        rewrite Forall_forall in H2...
+    - (* ite *)
+      destruct a; destruct is_control; repeat inv_bind; unfold normalize_ite;
+        repeat rewrite Forall_app; repeat split.
+      1,5: (eapply IHe; eauto).
+      1,2,4,5: (eapply map_bind2_untupled_eq; eauto; solve_forall).
+      rewrite Forall_forall; intros [? ?] Hin. rewrite map_map in Hin; simpl in Hin.
+      repeat simpl_In.
+      constructor. constructor.
+      + eapply normalized_lexp_hd_default.
+        eapply normalize_exp_normalized_lexp...
+      + eapply map_bind2_normalized_cexp in H2.
+        rewrite Forall_forall in H2...
+      + eapply map_bind2_normalized_cexp in H3.
+        rewrite Forall_forall in H3...
+    - (* app *)
+      eapply map_bind2_normalized_lexp in H1...
+      destruct ro; repeat inv_bind.
+      + specialize (normalize_reset_spec (hd_default x)) as [[? [? [? Hspec]]]|Hspec]; subst;
+          rewrite Hspec in H4; clear Hspec; repeat inv_bind.
+        * destruct x3...
+        * destruct (hd _) as [? [? ?]]; repeat inv_bind...
+      + constructor...
+    - (* app (auxiliary equations) *)
+      rewrite Forall_app. split.
+      + destruct ro; repeat inv_bind;
+        eapply map_bind2_untupled_eq in H1; eauto; solve_forall.
+      + destruct ro; repeat inv_bind; try constructor;
+        eapply Forall_app. split.
+        * eapply H in H2...
+        * specialize (normalize_reset_spec (hd_default x)) as [[? [? [? Hspec]]]|Hspec]; subst;
+          rewrite Hspec in H4; clear Hspec; repeat inv_bind...
+          destruct (hd _) as [? [? ?]]; repeat inv_bind.
+          repeat constructor. apply normalized_lexp_hd_default...
+  Qed.
+  Local Hint Resolve normalize_exp_untupled_eq.
+
+  Corollary normalize_exps_untupled_eq : forall es es' eqs' st st',
+      normalize_exps es st = (es', eqs', st') ->
+      Forall untupled_equation eqs'.
+  Proof.
+    intros * Hnorm.
+    unfold normalize_exps in Hnorm. repeat inv_bind.
+    eapply map_bind2_untupled_eq in H; eauto.
+    solve_forall.
+  Qed.
+  Local Hint Resolve normalize_exps_untupled_eq.
+
+  (* Intermediary predicate for normalized rhs *)
+  Inductive untupled_rhs : exp -> Prop :=
+  | untupled_rhs_Eapp : forall f es lann,
+      Forall normalized_lexp es ->
+      untupled_rhs (Eapp f es None lann)
+  | untupled_rhs_Eapp_reset : forall f es x ty cl lann,
+      Forall normalized_lexp es ->
+      untupled_rhs (Eapp f es (Some (Evar x (ty, cl))) lann)
+  | untupled_rhs_Efby : forall e0 e ann,
+      normalized_lexp e0 ->
+      normalized_lexp e ->
+      untupled_rhs (Efby [e0] [e] [ann])
+  | untupled_rhs_cexp : forall e,
+      normalized_cexp e ->
+      untupled_rhs e.
+  Hint Constructors untupled_rhs.
+
+  Fact untupled_equation_untupled_rhs : forall xs es,
+      untupled_equation (xs, es) ->
+      Forall untupled_rhs es.
+  Proof with eauto.
+    intros * Hnormed.
+    inv Hnormed...
+  Qed.
+
+  Fact normalize_rhs_untupled_rhs : forall e es' eqs' st st',
+      normalize_rhs e st = (es', eqs', st') ->
+      Forall untupled_rhs es'.
+  Proof with eauto.
+    intros * Hnorm.
+    destruct e; unfold normalize_rhs in Hnorm;
+      try (apply normalize_exp_normalized_cexp in Hnorm; solve_forall; auto).
+    - (* fby *)
+      repeat inv_bind.
+      apply normalize_exps_normalized_lexp in H.
+      apply normalize_exps_normalized_lexp in H0.
+      unfold normalize_fby.
+      apply Forall_forall; intros * Hin.
+      repeat simpl_In.
+      constructor.
+      + eapply Forall_forall in H3; eauto.
+      + eapply Forall_forall in H1; eauto.
+    - (* app *)
+      destruct o; repeat inv_bind...
+      specialize (normalize_reset_spec (hd_default x4)) as [[? [[? ?] [? Hspec]]]|Hspec]; subst;
+        rewrite Hspec in H1; clear Hspec; repeat inv_bind...
+      destruct (hd _) as [? [ty cl]]; repeat inv_bind...
+  Qed.
+
+  Corollary normalize_rhss_untupled_rhs : forall es es' eqs' st st',
+      normalize_rhss es st = (es', eqs', st') ->
+      Forall untupled_rhs es'.
+  Proof with eauto.
+    intros * Hnorm.
+    unfold normalize_rhss in Hnorm. repeat inv_bind.
+    eapply map_bind2_values in H.
+    induction H; simpl; try constructor.
+    apply Forall_app. split; auto.
+    destruct H as [? [? H]].
+    eapply normalize_rhs_untupled_rhs; eauto.
+  Qed.
+
+  Fact normalize_rhs_untupled_eq : forall e es' eqs' st st',
+      normalize_rhs e st = (es', eqs', st') ->
+      Forall untupled_equation eqs'.
+  Proof with eauto.
+    intros * Hnorm.
+    destruct e; unfold normalize_rhs in Hnorm;
+      try (eapply normalize_exp_untupled_eq in Hnorm; eauto).
+    - (* fby *)
+      repeat inv_bind.
+      repeat rewrite Forall_app. repeat split...
+    - (* app *)
+      repeat inv_bind...
+      destruct o; repeat inv_bind; repeat rewrite Forall_app; repeat split...
+      specialize (normalize_reset_spec (hd_default x4)) as [[? [? [? Hspec]]]|Hspec]; subst;
+        rewrite Hspec in H1; clear Hspec; repeat inv_bind; eauto.
+      + destruct (hd _ _) as [? [? ?]]; simpl in H1.
+        repeat inv_bind. repeat constructor.
+        apply normalized_lexp_hd_default...
+  Qed.
+  Hint Resolve normalize_rhs_untupled_eq.
+
+  Corollary normalize_rhss_untupled_eq : forall es es' eqs' st st',
+      normalize_rhss es st = (es', eqs', st') ->
+      Forall untupled_equation eqs'.
+  Proof.
+    intros * Hnorm.
+    unfold normalize_rhss in Hnorm; repeat inv_bind.
+    eapply map_bind2_untupled_eq in H; eauto.
+    rewrite Forall_forall; intros; eauto.
+  Qed.
+  Hint Resolve normalize_rhss_untupled_eq.
+
+  Lemma untuple_equation_untupled_eq : forall G eq eqs' st st',
+      wl_equation G eq ->
+      untuple_equation eq st = (eqs', st') ->
+      Forall untupled_equation eqs'.
+  Proof with eauto.
+    intros G [xs es] * Hwl Hnorm.
+    unfold untuple_equation in Hnorm.
+    repeat inv_bind.
+    rewrite Forall_app. split.
+    - assert (length xs = length (annots x)) as Hlen.
+      { destruct Hwl as [Hwl1 Hwl2].
+        eapply normalize_rhss_annots_length in H...
+        congruence. } clear Hwl.
+      eapply normalize_rhss_untupled_rhs in H; eauto.
+      revert xs Hlen.
+      induction H; intros xs Hlen; constructor.
+      + inv H...
+        * destruct xs; simpl in *; try omega.
+          constructor...
+        * simpl in Hlen. rewrite app_length in Hlen.
+          rewrite length_annot_numstreams in Hlen.
+          specialize (normalized_cexp_numstreams _ H1) as Hlen'.
+          rewrite Hlen' in *. simpl.
+          destruct xs... simpl in Hlen. omega.
+      + eapply IHForall.
+        rewrite skipn_length.
+        rewrite Hlen. simpl. rewrite app_length.
+        rewrite length_annot_numstreams. omega.
+    - eapply normalize_rhss_untupled_eq in H; eauto.
+  Qed.
+
+  Corollary untuple_equations_untupled_eq : forall G eqs eqs' st st',
+      Forall (wl_equation G) eqs ->
+      untuple_equations eqs st = (eqs', st') ->
+      Forall untupled_equation eqs'.
+  Proof.
+    induction eqs; intros * Hwl Hnorm;
+      unfold untuple_equations in Hnorm; repeat inv_bind; simpl; auto.
+    inv Hwl. apply Forall_app; split.
+    - eapply untuple_equation_untupled_eq; eauto.
+    - eapply IHeqs; eauto.
+      unfold untuple_equations; repeat inv_bind; repeat eexists; eauto.
+      inv_bind; eauto.
+  Qed.
+
+  (** ** No anonymous names in a normalized node *)
+
+  Fact normalized_lexp_no_fresh : forall e,
+      normalized_lexp e ->
+      fresh_in e = [].
+  Proof with eauto.
+    intros e Hnormed.
+    induction Hnormed; simpl...
+    - (* binop *)
+      rewrite IHHnormed1. rewrite IHHnormed2. reflexivity.
+    - (* when *)
+      rewrite IHHnormed. reflexivity.
+  Qed.
+
+  Corollary normalized_lexps_no_fresh : forall es,
+      Forall normalized_lexp es ->
+      fresh_ins es = [].
+  Proof.
+    induction es; intros; auto.
+    unfold fresh_ins in *; simpl.
+    inv H. rewrite IHes, app_nil_r; auto using normalized_lexp_no_fresh.
+  Qed.
+
+  Fact normalized_cexp_no_fresh : forall e,
+      normalized_cexp e ->
+      fresh_in e = [].
+  Proof with eauto.
+    intros e Hnormed.
+    induction Hnormed; simpl...
+    - (* merge *)
+      rewrite IHHnormed1. rewrite IHHnormed2. reflexivity.
+    - (* ite *)
+      rewrite IHHnormed1. rewrite IHHnormed2.
+      rewrite normalized_lexp_no_fresh...
+    - (* lexp *)
+      eapply normalized_lexp_no_fresh...
+  Qed.
+
+  Corollary normalized_cexps_no_fresh : forall es,
+      Forall normalized_cexp es ->
+      fresh_ins es = [].
+  Proof.
+    induction es; intros; auto.
+    unfold fresh_ins in *; simpl.
+    inv H. rewrite IHes, app_nil_r; auto using normalized_cexp_no_fresh.
+  Qed.
+
+  Corollary normalize_exp_no_fresh : forall e is_control es' eqs' st st',
+      normalize_exp is_control e st = (es', eqs', st') ->
+      fresh_ins es' = [].
+  Proof.
+    intros e is_control es' eqs' st st' Hnorm.
+    unfold fresh_ins. rewrite concat_eq_nil, Forall_map.
+    destruct is_control.
+    - apply normalize_exp_normalized_cexp in Hnorm.
+      eapply Forall_impl; eauto. intros. apply normalized_cexp_no_fresh; auto.
+    - apply normalize_exp_normalized_lexp in Hnorm.
+      eapply Forall_impl; eauto. intros. apply normalized_lexp_no_fresh; auto.
+  Qed.
+
+  Corollary normalize_reset_no_fresh : forall e e' eqs' st st',
+      normalize_reset e st = (e', eqs', st') ->
+      fresh_in e' = [].
+  Proof.
+    intros * Hnorm.
+    apply normalize_reset_normalized_lexp, normalized_lexp_no_fresh in Hnorm; auto.
+  Qed.
+
+  Corollary normalize_exps_no_fresh : forall es es' eqs' st st',
+      normalize_exps es st = (es', eqs', st') ->
+      fresh_ins es' = [].
+  Proof.
+    induction es; intros es' eqs' st st' Hnorm;
+      unfold fresh_ins;
+      unfold normalize_exps in Hnorm; repeat inv_bind; auto.
+    simpl. rewrite map_app, concat_app.
+    eapply normalize_exp_no_fresh in H.
+    unfold fresh_ins in H, IHes; rewrite H; simpl.
+    eapply IHes.
+    unfold normalize_exps; inv_bind.
+    repeat eexists; eauto. inv_bind; eauto.
+  Qed.
+
+  Fact untupled_equation_no_anon_in_eq : forall e,
+      untupled_equation e ->
+      anon_in_eq e = [].
+  Proof with eauto.
+    intros * Hnormed.
+    induction Hnormed; unfold anon_in_eq, anon_ins; simpl; repeat rewrite app_nil_r.
+    - (* app *)
+      unfold fresh_ins. rewrite concat_eq_nil, Forall_map.
+      solve_forall. eapply normalized_lexp_no_fresh...
+    - (* app (reset) *)
+      unfold fresh_ins. rewrite concat_eq_nil, Forall_map.
+      solve_forall. eapply normalized_lexp_no_fresh...
+    - (* fby *)
+      rewrite normalized_lexp_no_fresh...
+      rewrite normalized_lexp_no_fresh...
+    - (* cexp *)
+      specialize (anon_in_fresh_in e) as Hincl.
+      rewrite normalized_cexp_no_fresh in Hincl...
+      apply incl_nil...
+  Qed.
+
+  Lemma untupled_equations_no_anon : forall eqs,
+      Forall untupled_equation eqs ->
+      anon_in_eqs eqs = [].
+  Proof.
+    intros * Hnormed.
+    unfold anon_in_eqs.
+    rewrite concat_eq_nil, Forall_map.
+    solve_forall. eapply untupled_equation_no_anon_in_eq; eauto.
+  Qed.
+
+  Corollary untuple_equations_no_anon : forall G eqs eqs' st st',
+      Forall (wl_equation G) eqs ->
+      untuple_equations eqs st = (eqs', st') ->
+      anon_in_eqs eqs' = [].
+  Proof.
+    intros * Hwl Hnorm.
+    eapply untupled_equations_no_anon.
+    eapply untuple_equations_untupled_eq; eauto.
+  Qed.
+
+  (** ** Normalization of a full node *)
+
+  Import Fresh Fresh.Fresh Facts Tactics.
+
+  Definition untuple_equations' (eq : list equation) (st : fresh_st (type * clock)) :
+    { res | untuple_equations eq st = res }.
+  Proof.
+    remember (untuple_equations eq st) as eqs'.
+    econstructor; eauto.
+  Defined.
+
+  Definition first_unused_ident (vs : list ident) : ident :=
+    ((fold_left Pos.max vs xH) + 100)%positive.
+
+  Fact first_unused_ident_gt : forall vs id,
+      first_unused_ident vs = id ->
+      Forall (fun id' => (id' < id)%positive) vs.
+  Proof.
+    intros n id Hfirst.
+    subst. unfold first_unused_ident.
+    rewrite Forall_forall; intros x Hin.
+    eapply Pos.le_lt_trans. 2: apply Pos.lt_add_r.
+    apply max_fold_in; auto.
+  Qed.
+
+  Program Definition untuple_node (n : node) (G : { G | wl_node G n}) : node :=
+    let anon := anon_in_eqs (n_eqs n) in
+    let id0 := first_unused_ident (reserved++List.map fst (n_in n++n_vars n++n_out n++anon)) in
+    let eqs := untuple_equations' (n_eqs n) (init_st id0) in
+    let nvars := (st_anns (snd (proj1_sig eqs))) in
+    {| n_name := (n_name n);
+       n_hasstate := (n_hasstate n);
+       n_in := (n_in n);
+       n_out := (n_out n);
+       n_vars := (n_vars n)++nvars;
+       n_eqs := fst (proj1_sig eqs);
+       n_ingt0 := (n_ingt0 n);
+       n_outgt0 := (n_outgt0 n);
+    |}.
+  Next Obligation.
+    remember (first_unused_ident _) as id0.
+    eapply untuple_equations_vars_perm with (st:=init_st id0) in H. 2: eapply surjective_pairing.
+    specialize (n_defd n) as Hperm'.
+    unfold st_ids, idty in *. rewrite init_st_anns in H. rewrite app_nil_r in H.
+    etransitivity. apply H.
+    rewrite Permutation_app_comm. symmetry.
+    rewrite <- app_assoc. rewrite Permutation_swap.
+    repeat rewrite map_app in *.
+    rewrite Hperm'. reflexivity.
+  Qed.
+  Next Obligation.
+    remember (first_unused_ident _) as id0.
+    specialize (first_unused_ident_gt _ id0 (eq_sym Heqid0)) as Hident.
+    remember (untuple_equations (n_eqs n) (init_st id0)) as res.
+    assert (st_valid_reuse (snd res) (PSP.of_list (map fst (n_in n ++ n_vars n ++ n_out n)))
+                           PS.empty) as Hvalid.
+    { specialize (n_nodup n) as Hndup. rewrite fst_NoDupMembers in Hndup.
+      repeat rewrite map_app in Hndup.
+      subst. eapply untuple_equations_st_valid.
+      2: eapply surjective_pairing.
+      2: eapply init_st_valid_reuse.
+      + rewrite PSP.elements_empty, app_nil_r.
+        repeat ndup_r Hndup.
+      + replace (ps_adds _ PS.empty) with (ps_from_list (map fst (anon_in_eqs (n_eqs n)))); auto.
+        rewrite ps_from_list_ps_of_list.
+        repeat rewrite ps_of_list_ps_to_list_Perm; repeat rewrite map_app; repeat rewrite <- app_assoc in *; auto.
+        repeat ndup_r Hndup.
+        repeat rewrite app_assoc in Hndup. apply NoDup_app_l in Hndup.
+        repeat rewrite <- app_assoc in Hndup; auto.
+      + rewrite <- ps_from_list_ps_of_list. rewrite PS_For_all_Forall'.
+        eapply Forall_incl; eauto.
+        repeat rewrite map_app.
+        repeat apply incl_tl.
+        repeat rewrite app_assoc. apply incl_appl. reflexivity.
+      + replace (ps_adds _ PS.empty) with (ps_from_list (map fst (anon_in_eqs (n_eqs n)))); auto.
+        rewrite PS_For_all_Forall'.
+        eapply Forall_incl; eauto.
+        repeat rewrite map_app.
+        repeat apply incl_tl.
+        repeat apply incl_appr. reflexivity. }
+    destruct res as [eqs st']. simpl in *.
+    apply st_valid_reuse_st_valid in Hvalid. apply st_valid_NoDup in Hvalid.
+    specialize (n_nodup n) as Hndup.
+    rewrite ps_of_list_ps_to_list_Perm in Hvalid.
+    - rewrite fst_NoDupMembers.
+      repeat rewrite map_app in *.
+      unfold idty, st_ids in *; simpl.
+      rewrite <- app_assoc, app_assoc, Permutation_swap, <- app_assoc.
+      assert (anon_in_eqs eqs = []).
+      { symmetry in Heqres. eapply untuple_equations_no_anon in Heqres; eauto. }
+      rewrite H0; simpl. rewrite app_nil_r. assumption.
+    - rewrite <- fst_NoDupMembers.
+      repeat rewrite app_assoc in *.
+      apply NoDupMembers_app_l in Hndup; auto.
+  Qed.
+  Admit Obligations.
+
+  Fixpoint untuple_global (G : global) (Hwl: wl_global G) : global.
+  Proof.
+    destruct G as [|hd tl].
+    - exact [].
+    - refine ((untuple_node hd _)::(untuple_global tl _)).
+      + econstructor. inv Hwl; eauto.
+      + inv Hwl; eauto.
+  Defined.
+
+  (** *** After normalization, a global is normalized *)
+
+  Lemma untuple_node_untupled_node : forall n Hwl,
+      untupled_node (untuple_node n Hwl).
+  Proof.
+    intros n [G Hwl].
+    unfold untuple_node.
+    unfold untupled_node; simpl.
+    eapply untuple_equations_untupled_eq; eauto.
+    apply surjective_pairing.
+  Qed.
+
+  Lemma untuple_global_untupled_global : forall G Hwl,
+      untupled_global (untuple_global G Hwl).
+  Proof.
+    induction G; intros Hwl; simpl; constructor.
+    - apply untuple_node_untupled_node.
+    - apply IHG.
+  Qed.
+
+  (** *** untuple_global produces an equivalent global *)
+
+  Fact untuple_global_eq : forall G Hwt,
+      global_iface_eq G (untuple_global G Hwt).
+  Proof.
+    induction G; intros Hwt.
+    - reflexivity.
+    - simpl. apply global_iface_eq_cons; auto.
+  Qed.
+
+  Fact untuple_global_names : forall a G Hwt,
+      Forall (fun n => (n_name a <> n_name n)%type) G ->
+      Forall (fun n => (n_name a <> n_name n)%type) (untuple_global G Hwt).
+  Proof.
+    induction G; intros Hwt Hnames; simpl.
+    - constructor.
+    - inv Hnames.
+      constructor; eauto.
+  Qed.
+
+  (** ** Additional properties *)
+
+  Fact idents_for_anns'_anon_streams : forall anns ids st st',
+      idents_for_anns' anns st = (ids, st') ->
+      incl (anon_streams anns) (anon_streams (map snd ids)).
+  Proof.
+    induction anns; intros ids st st' Hids;
+      repeat inv_bind; simpl; auto.
+    - reflexivity.
+    - destruct a as [ty [cl [name|]]]; repeat inv_bind; simpl in *.
+      + apply incl_tl'; eauto.
+      + eauto.
+  Qed.
+
+  Definition without_names' (vars : list (ident * ann)) : list (ident * (Op.type * clock)) :=
+    List.map (fun '(id, (ty, (cl, _))) => (id, (ty, cl))) vars.
+
+  Fact idents_for_anns'_anon_streams_incl : forall anns ids st st',
+      idents_for_anns' anns st = (ids, st') ->
+      incl (anon_streams anns) (without_names' ids).
+  Proof.
+    induction anns; intros ids st st' Hids;
+      repeat inv_bind; simpl; try reflexivity.
+    destruct a as [ty [cl [name|]]]; repeat inv_bind; simpl.
+    - eapply incl_tl'; eauto.
+    - eapply incl_tl; eauto.
+  Qed.
+
+  (** ** fresh_ins appear in the state after normalisation *)
+
+  Fact map_bind2_fresh_incl : forall is_control es es' eqs' st st',
+      Forall (fun e => forall es' eqs' st st',
+                normalize_exp is_control e st = (es', eqs', st') ->
+                incl (fresh_in e) (st_anns st')) es ->
+      map_bind2 (normalize_exp is_control) es st = (es', eqs', st') ->
+      incl (fresh_ins es) (st_anns st').
+  Proof with eauto.
+    induction es; intros es' eqs' st st' Hf Hmap;
+      repeat inv_bind; try apply incl_nil'.
+    inv Hf.
+    apply incl_app; eauto.
+    etransitivity; eauto.
+    apply st_follows_incl; repeat solve_st_follows.
+  Qed.
+
+  Fact idents_for_anns'_fresh_incl : forall anns ids st st',
+      idents_for_anns' anns st = (ids, st') ->
+      incl (anon_streams anns) (st_anns st').
+  Proof.
+    intros anns ids st st' Hids.
+    etransitivity. eapply idents_for_anns'_anon_streams_incl; eauto.
+    eapply idents_for_anns'_incl; eauto.
+  Qed.
+
+  Fact normalize_exp_fresh_incl : forall e is_control es' eqs' st st',
+      normalize_exp is_control e st = (es', eqs', st') ->
+      incl (fresh_in e) (st_anns st').
+  Proof with eauto.
+    induction e using exp_ind2; intros is_control es' eqs' st st' Hnorm;
+      repeat inv_bind; eauto.
+    - (* const *) apply incl_nil'.
+    - (* var *) apply incl_nil'.
+    - (* binop *)
+      apply incl_app; eauto.
+      etransitivity...
+    - (* fby *)
+      apply incl_app.
+      + assert (st_follows x1 st') by repeat solve_st_follows.
+        apply map_bind2_fresh_incl in H1. 2:solve_forall.
+        etransitivity...
+      + assert (st_follows x4 st') by repeat solve_st_follows.
+        apply map_bind2_fresh_incl in H2. 2:solve_forall.
+        etransitivity...
+    - (* when *)
+      destruct a; repeat inv_bind.
+      apply map_bind2_fresh_incl in H0... solve_forall.
+    - (* merge *)
+      destruct a; repeat inv_bind.
+      assert (st_follows x2 x5) by repeat solve_st_follows.
+      apply map_bind2_fresh_incl in H1.
+      apply map_bind2_fresh_incl in H2. 2,3:solve_forall.
+      assert (st_follows x5 st').
+      { destruct is_control; repeat inv_bind; repeat solve_st_follows. }
+      eapply incl_app; etransitivity; eauto. etransitivity...
+    - (* ite *)
+      destruct a; repeat inv_bind.
+      assert (st_follows x1 x4) by repeat solve_st_follows.
+      assert (st_follows x4 x7) by repeat solve_st_follows.
+      eapply IHe in H1.
+      eapply map_bind2_fresh_incl in H2.
+      eapply map_bind2_fresh_incl in H3. 2,3:solve_forall.
+      assert (st_follows x7 st').
+      { destruct is_control; repeat inv_bind; repeat solve_st_follows. }
+      repeat eapply incl_app; repeat (etransitivity; eauto).
+    - (* app *)
+      apply map_bind2_fresh_incl in H1. 2:solve_forall.
+      assert (st_follows x1 st').
+      { destruct ro; repeat inv_bind; repeat solve_st_follows. }
+      destruct ro; repeat inv_bind; repeat eapply incl_app.
+      1,4:etransitivity; eauto; eapply incl_map; etransitivity; eauto; reflexivity.
+      2,3:eapply idents_for_anns'_fresh_incl...
+      assert (st_follows x8 st') by repeat solve_st_follows.
+      etransitivity...
+  Qed.
+
+  Corollary map_bind2_normalize_exp_fresh_incl : forall es is_control es' eqs' st st',
+      map_bind2 (normalize_exp is_control) es st = (es', eqs', st') ->
+      incl (fresh_ins es) (st_anns st').
+  Proof.
+    intros es is_control es' eqs' st st' Hmap.
+    apply map_bind2_fresh_incl in Hmap; auto.
+    solve_forall. apply normalize_exp_fresh_incl in H0; auto.
+  Qed.
+
+  Corollary normalize_exps_fresh_incl : forall es es' eqs' st st',
+      normalize_exps es st = (es', eqs', st') ->
+      incl (fresh_ins es) (st_anns st').
+  Proof.
+    intros es es' eqs' st st' Hnorm.
+    unfold normalize_exps in Hnorm; repeat inv_bind.
+    apply map_bind2_normalize_exp_fresh_incl in H; auto.
+  Qed.
+
+  (** ** Preservation of clockof *)
+
+  Fact normalize_exp_clockof : forall G e is_control es' eqs' st st',
+      wl_exp G e ->
+      normalize_exp is_control e st = (es', eqs', st')  ->
+      clocksof es' = clockof e.
+  Proof with eauto.
+    intros vars e is_control es' eqs' st st' Hwl Hnorm.
+    eapply normalize_exp_annot in Hnorm...
+    rewrite clocksof_annots, Hnorm, <- clockof_annot...
+  Qed.
+  Hint Resolve normalize_exp_clockof.
+End UNTUPLE.
+
+Module UntupleFun
+       (Ids : IDS)
+       (Op : OPERATORS)
+       (OpAux : OPERATORS_AUX Op)
+       (Syn : LSYNTAX Ids Op)
+       <: UNTUPLE Ids Op OpAux Syn.
+  Include UNTUPLE Ids Op OpAux Syn.
+End UntupleFun.
